moved current version to Session.v.  removed previous module iterations in Session.v

Session.v
@@ -3,977 +3,26 @@ Require Export CpdtTactics.
 Require Export Setoid.
 Require Export Crypto.
 
-Module try1.
-
-Inductive ProtoA : Type :=
-| SendA : forall (A:Type), ProtoA -> ProtoA
-| RecA : forall (A:Type), ProtoA -> ProtoA
-| ChoiceA : ProtoA -> ProtoA -> ProtoA
-| OfferA : ProtoA -> ProtoA -> ProtoA
-| Eps : ProtoA.
-
-Notation "x :!: y" := (SendA x y)
-                          (at level 50, left associativity).
-
-Notation "x :?: y" := (RecA x y)
-                        (at level 50, left associativity).
-
-Notation "x :+: y" := (ChoiceA x y)
-                        (at level 50, left associativity).
-
-Notation "x :&: y" := (OfferA x y)
-                          (at level 50, left associativity).
-
-Check (nat :!: (bool :?: Eps)).
-
-Inductive Dual : ProtoA -> ProtoA -> Prop :=
-| senRec : forall (A:Type) (R S : ProtoA),
-    Dual R S -> Dual (A :!: R) (A :?: S)
-| recSen : forall (A:Type) (R S : ProtoA),
-    Dual R S -> Dual (A :?: R) (A :!: S)
-| choiceOffer : forall (R S T U: ProtoA),
-    Dual R S -> Dual T U -> Dual (R :+: T) (S :&: U)
-| offerChoice : forall (R S T U: ProtoA),
-    Dual R S -> Dual T U -> Dual (R :&: T) (S :+: U)
-| epsDual : Dual Eps Eps.
-
-Example dual1 : Dual (nat :!: Eps) (nat :?: Eps).
-Proof.
-  apply senRec.
-  apply epsDual.
-Qed.
-
-Hint Constructors Dual.
-
-Example dual2 : Dual (nat :!: (bool :?: Eps)) (nat :?: (bool :!: Eps)).
-Proof. auto. Qed.
-
-Example dual3 : Dual ((nat :!: (bool :?: Eps)) :+: (bool :!: (nat :?: Eps)))
-                     ((nat :?: (bool :!: Eps)) :&: (bool :?: (nat :!: Eps))).
-Proof. auto. Qed.
-
-(* How can we make the type of send more expressive?  It should be something like (a :!: r) -> r *)
-Inductive Session (P P':ProtoA) (T:Type) :=
-| send {A:Type} :  A -> Session P P' T.
-
-
-Check (Session (nat :!: Eps) (nat :?: Eps) nat).
-
-End try1.
-
-
-Module try2.
-
-Inductive sendT (A:Type) (R:Type) :=.
-Inductive recieveT (A:Type) (R:Type) :=.
-Inductive choiceT (R:Type) (S:Type) :=.
-Inductive offerT (R:Type) (S:Type) :=.
-
-Notation "x :!: y" := (sendT x y)
-                          (at level 50, left associativity).
-
-Notation "x :?: y" := (recieveT x y)
-                        (at level 50, left associativity).
-
-Notation "x :+: y" := (choiceT x y)
-                        (at level 50, left associativity).
-
-Notation "x :&: y" := (offerT x y)
-                        (at level 50, left associativity).
-
-(*Definition send {A:Type} {R:Type} : (A :!: R) -> A -> R := *)
-
-End try2.
-
-Module try3.
-
-(* Protocol expressions *)
-Inductive PExp : Set :=
-| Nat  : nat -> PExp
-| Plus : PExp -> PExp -> PExp
-| Send : PExp -> PExp -> PExp
-| Rec :  PExp -> PExp -> PExp
-| Eps : PExp.
-(*| Bool : bool -> PExp
-| And : PExp -> PExp -> PExp *)
-
-(* Protocol Types *)
-Inductive PType : Type :=
-| TNat
-| TEps
-| TSend : PType -> PType -> PType
-| TRec :  PType -> PType -> PType.
-
-Inductive hasType : PExp -> PType -> Prop :=
-| HtNat : forall n, hasType (Nat n) TNat
-| HtEps : hasType Eps TEps
-| HtPlus : forall e1 e2, hasType e1 TNat ->
-                    hasType e2 TNat ->
-                    hasType (Plus e1 e2 ) TNat
-| HtSend : forall e1 e2 t1 t2, hasType e1 t1 ->
-                       hasType e2 t2 ->
-                       hasType (Send e1 e2) (TSend t1 t2)
-| HtRec : forall e1 e2 t1 t2,  hasType e1 TNat ->
-                       hasType e2 t1 ->
-                       hasType (Rec e1 e2) (TRec t1 t2).
-
-
-
-Notation "x :!: y" := (Send x y)
-                          (at level 50, left associativity).
-
-Notation "x :?: y" := (Rec x y)
-                        (at level 50, left associativity).
-
-Notation "x ! y" := (TSend x y)
-                          (at level 50, left associativity).
-
-Notation "x ? y" := (TRec x y)
-                      (at level 50, left associativity).
-
-Notation "x :T: y" := (hasType x y)
-                       (at level 50, left associativity).
-
-Check ((Nat 4) :!: Eps).
-
-Definition Session (a:PType) (b:PType) := (a, b).
-
-(*Definition send {A:Type} {a r : PType} : A -> (Session (a ! r) (r)) -> nat := 3. *)
-
-Hint Constructors hasType.
-
-Example sendWellTyped1 : hasType ((Nat 4) :!: Eps) (TNat ! TEps).
-Proof. auto. Qed.
-
-Example sendWellTyped1' : ((Nat 4) :!: Eps) :T: (TNat ! TEps).
-Proof. auto. Qed.
-
-Example sendWellTyped2 : ((Plus (Nat 3) (Nat 1)) :!: Eps) :T: (TNat ! TEps).
-Proof. auto. Qed.
-
-Example sendWellTypedConcerning : ((Nat 4) :!: (Nat 4)) :T: (TNat ! TNat).
-Proof. eauto. Qed.
-
-
-Inductive Dual : PType -> PType -> Prop :=
-| senRec : forall a r s,
-    Dual r s -> Dual (a ! r) (a ? s)
-| recSen : forall a r s,
-    Dual r s -> Dual (a ? r) (a ! s)
-(*| choiceOffer : forall r s t u,
-    Dual r s -> Dual t u -> Dual (r :+: t) (s :&: u)
-| offerChoice : forall r s t u
-    Dual r s -> Dual t u -> Dual (r :&: t) (s :+: u) *)
-| natDual : Dual TNat TNat
-| epsDual : Dual TEps TEps.
-
-Hint Constructors Dual.
-
-
-Example simpleDual : Dual (TNat ! TEps) (TNat ? TEps).
-Proof. eauto. Qed.
-
-Definition sendNat (n:nat) := (Nat n :!: Eps).
-Check sendNat.
-
-Example sendNatType : forall n, hasType (sendNat n) (TNat ! TEps).
-Proof. unfold sendNat. eauto. Qed.
-
-Example existsDual' : forall p1 t1, hasType p1 t1 -> exists p2 t2, and (hasType p2 t2) (Dual t1 t2).
-Proof.
-  eauto. Abort.
-
-Example existsDual' : forall p1 t1, hasType p1 t1 -> exists p2 t2, and (hasType p2 t2) (Dual t1 t2).
-Proof.
-  intros. inversion H. subst. exists (Nat 1). exists TNat. split; eauto.
-  Abort. (*exists (Eps). exists TEps. split; eauto. subst.
-  exists (Nat 1). exists TNat. split; eauto.
-  exists (e1 :?: e2). exists (t0 ? t2). split. apply HtRec. destruct t0. apply H0.
-Qed. *)
-
-Example dualUnique : forall t1 t2 t3, and (Dual t1 t2) (Dual t1 t3) -> t2 = t3.
-Proof. eauto. Abort.
-
-
-
-End try3.
-
-Module try4.
-
-Definition SendT (A:Type) (R:Type) :=
-  fun (x:A) => R.
-
-    
-Inductive EpsT := epsC.
-
-
-Check SendT nat EpsT.
-
-(*Inductive ProtoT (R:Type) : Type :=
-| sendC {A:Type} : SendT A (ProtoT R) -> ProtoT R
-| receiveC {A:Type} : RecT A (ProtoT R) -> ProtoT R.
-
-Check sendC EpsT (
-
-Check sendC nat (EpsT).
-
-Definition isSend : Prop 
-
-Definition send {A R :Type} (a:A) (p: (SendT A R)) : R := match p with end.
-
-Check send 3 _. *)
-
-
-End try4.
-
-Module try5.
-
-Inductive SendT (A:Type) (R:Type) : Type := sendC : A -> R -> SendT A R.
-Inductive RecT  (A:Type) (R:Type) : Type := recC : R -> RecT A R.
-Inductive EpsT := epsC.
-
-Notation "x :!: y" := (SendT x y)
-                        (at level 50, left associativity).
-
-Notation "x :?: y" := (RecT x y)
-                        (at level 50, left associativity).
-
-Eval compute in sendC nat EpsT.
-
-Definition send {A R :Type} (s : A :!: R) : R :=
-  match s with
-    sendC _ r => r
-  end.
-
-(* Should we account for the received value of type A here?  With the current implementation, it simply disappears.  Maybe it should return a pair:  (A,R) *)
-Definition receive {A R :Type} (s : A :?: R) : R :=
-  match s with
-    recC r => r
-  end.
-
-
-Definition proto1 := (sendC nat EpsT).
-Check proto1.
-
-Definition proto1Applied := proto1 3 epsC.
-Print proto1Applied.
-
-Definition afterSend := send proto1Applied.
-Eval compute in afterSend.
-
-Definition proto2 := (recC nat EpsT).
-Check proto2.
-
-Definition proto2Applied := proto2 epsC.
-Check proto2Applied.
-
-(* Where does the received value go after this application? *)
-Definition afterReceive := receive proto2Applied.
-Eval compute in afterReceive.
-
-Definition proto3 := sendC nat (RecT nat EpsT).
-Eval compute in proto3.
-
-Definition proto3Applied := proto3 1 proto2Applied.
-Eval compute in proto3Applied.
-
-Inductive Dual : Type -> Type -> Prop :=
-| senRec : forall a r s, Dual r s -> Dual (a :!: r) (a :?: s)
-| recSen : forall a r s, Dual r s -> Dual (a :?: r) (a :!: s)
-| dualEps : Dual EpsT EpsT.
-
-Hint Constructors Dual SendT RecT EpsT.
-
-Example dual1 : Dual (nat :!: EpsT) (nat :?: EpsT).
-Proof. auto. Qed.
-
-Example dual2 : Dual (nat :!: (nat :?: EpsT)) (nat :?: (nat :!: EpsT)).
-Proof. auto. Qed.
-
-End try5.
-
-Module try6.
-
-Inductive session : Type :=
-| epsC : session
-| sendC : forall (B:Type),  session -> session
-| receiveC : forall (B:Type), session -> session
-(*| choiceC : session -> session -> session
-| offerC : session -> session -> session*).
-
-Notation "x :!: y" := (sendC x y)
-                        (at level 50, left associativity).
-
-Notation "x :?: y" := (receiveC x y)
-                        (at level 50, left associativity).
-
-(*Notation "x :+: y" := (choiceC x y)
-                        (at level 50, left associativity).
-
-Notation "x :&: y" := (offerC x y)
-                        (at level 50, left associativity). *)
-
-Check sendC nat (receiveC bool epsC).
-
-Definition unwrap (s:session) (*(b:bool)*) : session :=
-  match s with
-  | epsC => s
-  | sendC B s' => s'
-  | receiveC B s' => s'
-  (*| choiceC r s => if (b) then r else s
-  | offerC r s => if (b) then r else s   *)                                  
-  end.
-
-Definition sendReady (s:session) (A:Type) : Prop :=
-  match s with
-  | epsC => False
-  | sendC A _ => True
-  | receiveC _ _ => False
-(*  | choiceC _ _ => False
-  | offerC _ _ => False *)
-  end.
-
-Definition receiveReady (s:session) (A:Type) : Prop :=
-  match s with
-  | epsC => False
-  | sendC A _ => False
-  | receiveC _ _ => True
-  (*| choiceC _ _ => False
-  | offerC _ _ => False  *)                
-  end.
-
-Check sendC nat (receiveC bool epsC).
-
-Definition trans (A:Type) (B:Type) := A -> B.
-Definition transEx : trans nat bool := (fun (x:nat) => true).
-
-Definition send {A:Type} (x:A) (s:session) : (sendReady s A) -> 
-  {u:session | u = unwrap(s)}.
-    refine
-      (fun p  =>
-      match s with 
-      | sendC _ u => _
-      | receiveC _ u => _
-      | epsC => _
-      end).
-    unfold sendReady in p. destruct s in p. contradiction. unfold unwrap. apply (exist _ epsC). reflexivity. contradiction.
-    unfold sendReady in p. destruct s in p. contradiction. unfold unwrap. apply (exist _ u). reflexivity. contradiction.
-    unfold sendReady in p. destruct s in p. contradiction. unfold unwrap. apply (exist _ u). reflexivity. contradiction.
-Defined.
-
-Definition send' {A:Type} {pa:A->Prop} (ss:{x:A | pa x}) (s:session) : (sendReady s A) -> 
-  {u:session | u = unwrap(s)}.
-    refine
-      (fun p  =>
-      match s with 
-      | sendC _ u => _
-      | receiveC _ u => _
-      | epsC => _
-      end).
-    unfold sendReady in p. destruct s in p. contradiction. unfold unwrap. apply (exist _ epsC). reflexivity. contradiction.
-    unfold sendReady in p. destruct s in p. contradiction. unfold unwrap. apply (exist _ u). reflexivity. contradiction.
-    unfold sendReady in p. destruct s in p. contradiction. unfold unwrap. apply (exist _ u). reflexivity. contradiction.
-Defined.
-
-(* TODO:  make the return type a sumor.  The left side returns the current return type: a subset type that represents the "rest" of the protocol.  The right side returns a proof that the input predicate on the (x:A) could not be proven.  Note, this may require putting an additional restriction on the input predicate that it is decidable. *)
-Definition receive {A:Type} (x:A) (s:session) : (receiveReady s A) -> 
-  {u:session | u = unwrap(s)}.
-    refine
-      (fun p  =>
-      match s with 
-      | sendC _ u => _
-      | receiveC _ u => _
-      | epsC => _
-      end).
-    unfold receiveReady in p. destruct s in p. contradiction. contradiction. unfold unwrap. apply (exist _ epsC). reflexivity. 
-    unfold receiveReady in p. destruct s in p. contradiction. contradiction. unfold unwrap. apply (exist _ u). reflexivity.
-    unfold receiveReady in p. destruct s in p. contradiction. contradiction. unfold unwrap. apply (exist _ u). reflexivity.
-Defined.
-
-Definition proto2 := sendC bool (sendC nat epsC).
-Print proto2.
-
-Example sendReady2 : sendReady proto2 bool. reflexivity. Qed.
-
-Eval compute in ((send true proto2) sendReady2).
-Eval compute in unwrap proto2.
-
-Definition proto1 := unwrap proto2.
-Eval compute in proto1.
-
-Example sendReady1 : sendReady proto1 nat. reflexivity. Qed.
-
-Eval compute in ((send 1 proto1) sendReady1).
-Eval compute in unwrap proto1.
-
-Inductive Dual : session -> session -> Prop :=
-| dualEps : Dual epsC epsC
-| senRec : forall A r s, Dual r s -> Dual (sendC A r) (receiveC A s)
-| recSen : forall A r s, Dual r s -> Dual (receiveC A s) (sendC A r).                                    
-
-Definition proto3 := receiveC bool (receiveC nat epsC).
-Print proto3.
-
-Hint Constructors Dual.
-Example dualExample : Dual proto2 proto3. unfold proto2. unfold proto3. auto. Qed.
-
-Example receiveReady3 : receiveReady proto3 bool. reflexivity. Qed.
-
-Eval compute in proj1_sig ((receive true proto3) receiveReady3).
-(*Eval compute in unwrap proto3. *)
-
-Definition proto4 := unwrap proto3.
-Eval compute in proto4.
-
-Example receiveReady4 : receiveReady proto4 nat. reflexivity. Qed.
-
-Eval compute in ((receive 1 proto4) receiveReady4).
-Eval compute in unwrap proto4.
-
-
-Definition proto2' := sendC bool (sendC nat epsC).
-Print proto2'.
-
-Example sendReady2' : sendReady proto2' bool. reflexivity. Qed.
-
-Definition proto2'Pred := (fun (x:bool) => True).
-Example proto2'PredProof : (proto2'Pred true). reflexivity. Qed.
-
-Eval compute in send' (exist proto2'Pred true proto2'PredProof) proto2 sendReady2'.
-Eval compute in unwrap proto2.
-
-Set Implicit Arguments.
-(*Variable A : Set. *)
-Inductive maybe (A : Set) (P : A -> Prop) : Set :=
-| Unknown : maybe P
-| Found : forall x : A, P x -> maybe P.
-
-Notation "{{ x | P }}" := (maybe (fun x => P)).
-Notation "??" := (Unknown ).
-Notation "[| x |]" := (Found _ x  _).
-
-Notation "x <- e1 ; e2" := (match e1 with
-| Unknown => ??
-| Found x _ => e2
-end)
-(right associativity, at level 60).
-  
-End try6.
-
-Module try7.
-
-Inductive VarT :=
-| VarC : nat -> VarT.
-  
-Definition key_val : Type := nat.
-
-(** Key types are [symmetric], [public] and [private]. *)
-Inductive keyType: Type :=
-| symmetric : key_val -> keyType
-| private : key_val -> keyType
-| public : key_val -> keyType.
-
-(** Basic messages held abstract.  Compound messages are keys, encrypted and
-  signed messages, hashes and pairs. *)
-
-Inductive message : Type :=
-| basic : nat -> message
-| var : nat -> message
-| key : keyType -> message
-| encrypt : message -> keyType -> message
-| sign : message -> keyType -> message
-| hash : message -> message
-| pair : message -> message -> message.
-
-
-(* 
-protoType is the type language for protocols.
-
-Var- Represents a placeholder(natural number-indexed variable) in a protocol.  The idea is that it will bring new things received into scope for the rest of the protocol.
-
-Eps- The empty protocol's type.
-
-TODO: What is the best way to make global data(keys, for example) available to the protocol?  Include an environment structure?
-*)
-  
-Inductive protoType : Type :=
-| Send : forall (A:Type), protoType -> protoType
-| Receive : forall (A:Type), protoType -> protoType
-| Choice : protoType -> protoType -> protoType
-| Offer : protoType -> protoType -> protoType                                  
-(*| Var : nat -> protoType  (* TODO:  Does Var belong in protoType?  If not, could it be left external and only referenced as an argument to ReceiveC(below)?. If so, should the natural number index stay in the type? *)  *)              
-| Eps : protoType.
-
-Inductive protoExp : protoType -> Type :=
-| SendC {A:Type} {p:protoType} : message -> (protoExp p) -> protoExp (Send A p)
-| ReceiveC (A:Type) {p:protoType}
-    : VarT -> (protoExp p) -> protoExp (Receive A p)          
-(*| VarC (n:nat) :  protoExp (Var n) *)
-| ChoiceC {r s: protoType}
-  : bool -> (protoExp r) -> (protoExp s) -> (protoExp (Choice r s))
-| OfferC {r s : protoType}
-  : (protoExp r) -> (protoExp s) -> (protoExp (Offer r s))    
-| EpsC : protoExp Eps.
-
-Inductive DualT : protoType -> protoType -> Prop :=
-| senRec : forall A r s, DualT r s -> DualT (Send A r) (Receive A s)
-| recSen : forall A r s, DualT r s -> DualT (Receive A s) (Send A r)
-| chOff : forall r s r' s', DualT r r' -> DualT s s' -> DualT (Choice r s) (Offer r' s')
-| offCh : forall r s r' s', DualT r r' -> DualT s s' -> DualT (Offer r' s') (Choice r s)                                                        
-| dualEps : DualT Eps Eps.
-
-Definition Dual {t t': protoType} (r:protoExp t) (s:protoExp t') : Prop :=
-  DualT t t'.
-
-Notation "x :!: y" := (Send x y)
-                        (at level 50, left associativity).
-Notation "x :!: y" := (protoExp (Send x y))
-                        (at level 50, left associativity).
-
-Notation "x :?: y" := (Receive x y)
-                        (at level 50, left associativity).
-Notation "x :?: y" := (protoExp (Receive x y))
-                        (at level 50, left associativity).
-
-Notation "x :+: y" := (Choice x y)
-                        (at level 50, left associativity).
-(*Notation "x :+: y" := (protoExp (Choice x y))
-                        (at level 50, left associativity). *)
-
-Notation "x :&: y" := (Offer x y)
-                        (at level 50, left associativity).
-Notation "x :&: y" := (protoExp (Offer x y))
-                        (at level 50, left associativity).
-
-
-Definition proto1 := SendC (A:=nat) (basic 1) EpsC.
-Eval compute in proto1.
-
-Definition proto2 := ReceiveC nat (VarC 1) EpsC.
-Eval compute in proto2.
-
-Definition protoChoiceValue := ChoiceC true proto1 (SendC (A:=nat) (basic 2) EpsC).
-Eval compute in protoChoiceValue.
-
-Definition protoOfferValue := OfferC (ReceiveC nat (VarC 1) EpsC) (ReceiveC bool (VarC 1) EpsC).
-Eval compute in protoOfferValue.
-
-Hint Constructors DualT.
-
-Example simpleDual : Dual proto1 proto2.
-Proof. unfold Dual. auto. Qed.
-
-Definition proto3 := SendC (A:=nat) (basic 1) proto2.
-Eval compute in proto3.
-
-
-(* 
-What should a protocol "produce"?(what is the return type of runProto?). 
--Can we determine what it produces by the session type alone?
--Is "what a protocol produces" simply what it adds to its environment(new things received)?  Is it a single primitive value?
--How do we capture not only "what" a protocol produces, but PROPERTIES about what it produces(proofs about message content, execution, etc.)
--How do we sequence and compose protocols (thread the result of one to the next)?
- *)
-
-
-
-Definition var_id : Type := nat.
-Definition env_val : Type := message.
-
-Inductive environment : Type :=
-| empty : environment
-| item : var_id -> env_val -> environment -> environment.
-
-Definition add (id:var_id) (m:env_val) (e:environment) : environment :=
-  item id m e.
-
-Fixpoint delete (id:var_id) (e:environment) : environment :=
-  match e with
-  | empty => empty
-  | item id' m e' => if( beq_nat id id') then (delete id e') else item id' m (delete id e')
-  end.
-
-Fixpoint retrieve (id:var_id) (e:environment) : option env_val := 
-  match e with
-  | empty => None
-  | item id' m e' =>
-    if (beq_nat id id')
-                    then Some m
-                    else retrieve id e'
-  end.
-
-Definition empty_env := empty.
-Definition env_1 := add 1 (basic 1) empty_env.
-Print env_1.
-Definition env_2 := add 2 (basic 2) env_1.
-Definition env_3 := add 2 (basic 3) env_2.
-Definition env_4 := delete 2 env_3.
-Eval compute in env_4.
-Definition env_5 := delete 1 env_3.
-Eval compute in env_5.
-Eval compute in retrieve 2 env_5.
-
-Fixpoint evalMessage (m:message) (e:environment) : option message :=
-  match m with
-  | basic n => Some (basic n)
-  | var v => retrieve v e
-  | key k => Some (key k)
-  | encrypt m' k' =>
-    match (evalMessage m' e) with
-    | Some m'' => Some (encrypt m'' k')
-    | None => None
-    end
-  | sign m' k' =>
-    match (evalMessage m' e) with
-    | Some m'' => Some (sign m'' k')
-    | None => None
-    end      
-  | hash m' =>
-    match (evalMessage m' e) with
-    | Some m'' => Some (hash m'')
-    | None => None
-    end
-  | pair m1 m2 =>
-    match (evalMessage m1 e) with
-    | Some m'' =>
-      match (evalMessage m2 e) with
-      | Some m''' => Some (pair m'' m''')
-      | None => None
-      end
-    | None => None
-    end
-      
-  end.
-
-  
-Fixpoint runProto' {t t' : protoType} (p1:protoExp t) (p2:protoExp t') (p1Env : environment) (p2Env : environment) : option (environment * environment) :=
-match p1 with
-| SendC _ _ a p1' =>
-  match p2 with
-  | ReceiveC _ _ v p2' =>
-    match v with
-    | VarC n =>
-      match (evalMessage a p1Env) with
-      | Some m => runProto' p1' p2' p1Env (add n m p2Env)
-      | None => None
-      end
-    end
-  | _ => None
-  end
-| ReceiveC _ _ v p1' =>
-  match p2 with
-  | SendC _ _ a p2' =>  
-    match v with
-    | VarC n =>
-      match (evalMessage a p2Env) with
-      | Some m => runProto' p1' p2' (add n m p1Env) p2Env
-      | None => None
-      end
-    end
-  | _ => None
-  end
-| ChoiceC _ _ b p1' p1'' =>
-  match p2 with
-  | OfferC _ _ p2' p2'' => if (b) then runProto' p1' p2' p1Env p2Env
-                             else runProto' p1'' p2'' p1Env p2Env
-  | _ => None
-  end
-| EpsC => Some (p1Env, p2Env)    
-| _ => None
-end.
-
-Definition runProto {t t' : protoType} (r:protoExp t) (s:protoExp t') (rEnv : environment) (sEnv : environment) (p:Dual r s) : option (environment * environment) := runProto' r s rEnv sEnv.
-
-Eval compute in runProto proto1 proto2 empty_env empty_env simpleDual.
-
-Definition proto1' := SendC (A:=bool) (basic 2)
-                      (ReceiveC bool (VarC 42) 
-                      EpsC).
-Check proto1'.
-
-Definition proto2' := ReceiveC bool (VarC 1)
-                      (SendC (A:=bool) (sign (var 1) (private 0))
-                      EpsC).
-Check proto2'.
-
-Example dual12' : Dual proto1' proto2'. unfold Dual. auto. Qed.
-
-Eval compute in runProto proto1' proto2' empty_env empty_env dual12'.
-
-Definition proto3' (b:bool) := ChoiceC b
-                             proto1'
-                             proto2'.
-
-Definition proto4' := OfferC
-                        proto2'
-                        proto1'.
-
-Example dual3'4' : Dual (proto3' true) proto4'. unfold Dual. auto. Qed.
-
-Eval compute in runProto (proto3' true) proto4' empty_env empty_env dual3'4'.
-
-(*Definition proto5 := ReceiveC bool (VarC 1)
-                     (proto3' (beq_nat (basic 2) (VarC 1))). *)
-
-Definition proto6 := SendC (A:=bool) (basic 2)
-                     proto4'.
-
-                     
-                     
-End try7.
-
-Module try8.
-
-Inductive protoType : Type :=
-| Send : forall (A:Type), protoType -> protoType
-| Receive : forall (A:Type), protoType -> protoType
-| Choice : protoType -> protoType -> protoType
-| Offer : protoType -> protoType -> protoType   
-| Eps : protoType.
-
-Inductive Either (A:Type) (B:Type) : Type :=
-| eLeft : A -> Either A B
-| eRight : B -> Either A B.
-
-Inductive protoExp : Type -> protoType -> Type :=
-| SendC {A B:Type} {p':protoType} : A -> (protoExp B p') -> protoExp B (Send A p')
-| ReceiveC {A B:Type} {p':protoType}: (A->(protoExp B p')) -> protoExp B (Receive A p') 
-| ChoiceC {R S:Type} (b:bool) {r s: protoType}
-  : (protoExp R r) -> (protoExp S s) -> (protoExp (if(b) then R else S) (Choice r s))
-| OfferC {r s : protoType} {R S:Type}
-  : (protoExp R r) -> (protoExp S s) -> (protoExp (Either R S) (Offer r s)) 
-| ReturnC {T:Type} : T -> protoExp T (Eps).
-
-Notation "x :!: y" := (Send x y)
-                        (at level 50, left associativity). 
-Notation "x :!: y" := (protoExp (Send x y))
-                        (at level 50, left associativity).
-
-Notation "x :?: y" := (Receive x y)
-                        (at level 50, left associativity).  
-Notation "x :?: y" := (protoExp (Receive x y))
-                        (at level 50, left associativity).
-
-Notation "x :+: y" := (Choice x y)
-                        (at level 50, left associativity).
-Notation "x :+: y" := (protoExp (Choice x y))
-                        (at level 50, left associativity). 
-
-Notation "x :&: y" := (Offer x y)
-                        (at level 50, left associativity).
-Notation "x :&: y" := (protoExp (Offer x y))
-                        (at level 50, left associativity).
-
-Inductive DualT : protoType -> protoType -> Prop :=
-| senRec (A:Type) : forall r s, DualT r s -> DualT (Send A r) (Receive A s)
-| recSen (A:Type) : forall r s, DualT r s -> DualT (Receive A s) (Send A r)
-| chOff : forall r s r' s', DualT r r' -> DualT s s' -> DualT (Choice r s) (Offer r' s')
-| offCh : forall r s r' s', DualT r r' -> DualT s s' -> DualT (Offer r' s') (Choice r s)                                                        
-| dualEps : DualT (Eps) (Eps).
-
-Definition Dual {t t': protoType} {T T' : Type} (r:protoExp T t) (s:protoExp T' t') : Prop :=
-  DualT t t'.
-
-Fixpoint NotDualT (p1:protoType) (p2:protoType) : Prop :=
-  match p1 with
-  | Send A p1' =>
-    match p2 with
-    | Receive B p2' => (A <> B) \/ (NotDualT p1' p2')
-    | _ => True
-    end
-  | Receive A p1' =>
-    match p2 with
-    | Send B p2' => (A <> B) \/ (NotDualT p1' p2')
-    | _ => True
-    end
-  | Choice p1' p1'' =>
-    match p2 with
-    | Offer p2' p2'' => (NotDualT p1' p2') \/ (NotDualT p1'' p2'')
-    | _ => True
-    end
-  | Offer p1' p1'' =>
-    match p2 with 
-    | Choice p2' p2'' => (NotDualT p1' p2') \/ (NotDualT p1'' p2'')
-    | _ => True
-    end
-  | Eps =>
-    match p2 with
-    | Eps => False
-    | _ => True
-    end
-  end.
-            
-Definition NotDual {t t' : protoType} {T T' : Type} (r:protoExp T t) (s:protoExp T' t') : Prop :=
-  NotDualT t t'.
-  
-
-
-Definition EpsC := ReturnC tt.
-Definition proto1 := SendC 1 EpsC.
-Check proto1.
-
-Definition proto2 :=
-  SendC 1
-  ( ReceiveC (fun x =>
-  ( ReceiveC (fun y =>
-  ( SendC (x + y)
-  ( EpsC)))))).                   
-Check proto2.
-
-Notation "'send' n ; p" := (SendC n p)
-                            (right associativity, at level 60).
-Notation "x <- 'receive' ; p " := (ReceiveC (fun x => p)) 
-                                    (right associativity, at level 60).
-
-Notation "'offer'" := OfferC.
-
-Notation "'choice'" := ChoiceC. 
-
-Definition proto1' :=
-  send 1;
-  EpsC.
-Check proto1'.
-
-Definition proto2' :=
-  send 1;
-  x <- receive;
-  y <- receive;
-  send (x + y);
-  EpsC.
-Check proto2'.
-
-Definition proto2'' :=
-  send 1;
-  x <- receive;
-  y <- receive;
-  send (andb x y); (* EpsC. *)
-  ReturnC 2. (*(andb x y).*)
-Check proto2''.
-
-Definition constNat (_:bool) : nat := 42.
-
-Definition proto3 :=
-  x <- receive;
-  send (x+3);
-  send x;
-  y <- receive;
-  ReturnC (T:=bool) y (*(constNat y)*).
-Check proto3.
-
-Definition proto4 :=
-  x <- receive;
-  send (x + 1);
-  ReturnC true. (*x.*)
-Check proto4.
-
-Definition proto5 :=
-  send 1;
-  x <- receive;
-  ReturnC (T:=nat) x.
-Check proto5.
-
-Definition proto6 :=
-  offer EpsC
-        proto5. Check proto6.
-
-Definition proto7 (b:bool) :=
-  choice b
-         EpsC
-         proto4. Check (proto7 true).
-
-Definition proto8 :=
-  offer EpsC
-        proto6. Check proto8.
-
-Definition proto9 (b:bool) (b':bool) :=
-  choice b
-         EpsC
-         (proto7 b'). Check proto9 false false.
-
-Hint Constructors DualT.
-
-Example dual45 : Dual proto4 proto5. Proof. unfold Dual. apply (recSen nat). apply (recSen nat). auto. Qed.
-
-Example dual67 : Dual proto6 (proto7 true). Proof. unfold Dual. apply offCh. auto. apply dual45. Qed.
-
-Example dual89 : Dual proto8 (proto9 false false). unfold Dual. apply offCh. auto. apply chOff. auto. apply dual45. Qed.
-
-Definition proto3' :=
-  send 1;
-  EpsC.  Check proto3'.
-
-Definition proto4' :=
-  x <- receive;
-  ReturnC (T:=bool) x. Check proto4'.
-
-Eval compute in NotDual proto3' proto4'.
-
-Example natNotBool : (nat <> bool). Abort.
-
-
-
- 
-(*Fixpoint runProto' t t' C D  (p1:protoExp C t) (p2:protoExp D t') (p:Dual p1 p2) : C.
-  refine (
-  match p1 in (protoExp ReturnType pType) return (ReturnType) with
-| SendC SentType CCC pt1' a _ =>
-  match p2 in (protoExp ReturnType2 pType2) with
-  | ReceiveC RecType Tp2 pt2' fff => runProto' pt1' pt2' _ Tp2 _ _ _(*(fff a)*) _
-  | _ => _
-  end
-| _ => _
-  end). destruct p. inversion p0. subst. destruct p. apply (runProto' p'0 p' _ _ X0 p3). apply (runProto' p'0 p' _ _ X0 p3). apply (runProto' p'0 p' _ _ X0 p3). apply (runProto' p'0 p' _ _ X0 p3). apply (runProto' p'0 p' _ _ X0 p3). destruct H0.
-
-  destruct p1. destruct p2. unfold Dual in d.
- 
-
-  end
-| ReceiveC _ _ _ f =>
-  match p2 with
-  | SendC A C _ a p2' => _ (*runProto' _ _ C D _ (*(f a)*) p2' _ *)
-  | _ => _
-  end
-| ChoiceC _ _ b _ _ p1' p1'' => 
-  match p2 with
-  | OfferC _ _ _ _ p2' p2'' => if (b) then _ (*runProto' _ _ C D p1' p2' _ *)
-                                 else _ (*runProto' _ _ C D p1'' p2'' _ *)
-  | _ => _
-  end
-| ReturnC A a => _ 
-| _ => _
-  end). destruct p1. destruct p2.  
-  unfold Dual in d. inversion d.
-
-Definition runProto {A:Type} {t t' : protoType} (r:protoExp t) (s:protoExp t') (p:Dual r s) : A  := runProto' r s. *)
-
-
-
-End try8.
-
-Module try9.
+Module session.
 
 Inductive protoType : Type :=
 | Send : type -> protoType -> protoType
 | Receive : type -> protoType -> protoType
 | Choice : protoType -> protoType -> protoType
-| Offer : protoType -> protoType -> protoType
-| Decrypt : protoType -> protoType                                    
+| Offer : protoType -> protoType -> protoType  
 | Eps : type -> protoType.
 
-(*Inductive Either (A:Type) (B:Type) : Type :=
-| eLeft : A -> Either A B
-| eRight : B -> Either A B. *)
 
+Definition t1 := Send (Basic) (Eps Basic). Check t1.
   
 Inductive protoExp : type -> protoType -> Type :=
-| SendC {t:type} {T:type} {p':protoType}  : (message t) -> (protoExp T p') -> protoExp T (Send t p')
-| ReceiveC {t:type} {T:type} {p':protoType} : ((message t)->(protoExp T p')) -> protoExp T  (Receive t p') 
-| ChoiceC (b:bool) {r s: protoType} {R S:type}
-  : (protoExp R r) -> (protoExp S s) -> (protoExp (if(b) then R else S) (Choice r s))
-| OfferC {r s : protoType} {R S:type}
-  : (protoExp R r) -> (protoExp S s) -> (protoExp (Either R S) (Offer r s))
-| DecryptC {p':protoType} {mt T:type} : (message (Encrypt mt)) ->
-                                        (protoExp T p') -> protoExp T (Decrypt p')   
+| SendC {t:type} {T:type} {p':protoType}  : (message t) -> (protoExp T p')
+    -> protoExp T (Send t p')
+| ReceiveC {t:type} {T:type} {p':protoType} : ((message t)->(protoExp T p'))     -> protoExp T  (Receive t p') 
+| ChoiceC (b:bool) {r s:protoType} {R S:type} :(protoExp R r) -> (protoExp S s)
+    -> (protoExp (if(b) then R else S) (Choice r s))
+| OfferC {r s : protoType} {R S:type} : (protoExp R r) -> (protoExp S s)
+    -> (protoExp (Either R S) (Offer r s))  
 | ReturnC {t:type} : (message t) -> protoExp t (Eps t).
 
 Notation "x :!: y" := (Send x y)
@@ -1012,102 +61,133 @@ Check proto1.
 Definition unwrapBasic (m:message Basic) : nat :=
   match m with
   | basic n => n
+  | _ => 0
   end.
 
 
-Definition proto2 :=
-  SendC (basic 1)
-  ( ReceiveC (fun x =>
-  ( ReceiveC (fun y =>
-  ( SendC (basic ((unwrapBasic x) + (unwrapBasic y)))
-  ( EpsC)))))).                   
-Check proto2.
+Definition enc1 := encrypt Basic (basic 42) (public 1). Check enc1.
+Definition enc2 := encrypt _ enc1 (public 2).
+Eval compute in decryptM enc1 (private 1).
+Eval compute in decryptM enc1 (private 0).
+Eval compute in decryptM enc2 (private 2).
+Eval compute in decryptM (decryptM enc2 (private 2)) (private 1).
 
-Check Prop.
-(*Inductive DualT : protoType -> protoType -> Prop :=
-| senRec : forall t r s, DualT r s -> DualT (Send t r) (Receive t s)
-| recSen : forall t r s, DualT r s -> DualT (Receive t s) (Send t r)
-| chOff : forall r s r' s', DualT r r' -> DualT s s' -> DualT (Choice r s) (Offer r' s')
-| offCh : forall r s r' s', DualT r r' -> DualT s s' -> DualT (Offer r' s') (Choice r s)                                                        
-| dualEps : forall t,  DualT (Eps t) (Eps t). *)
-
-(*Definition Dual {t t': protoType}{T T':type} (r:protoExp T t) (s:protoExp T' t') : Prop :=
-  DualT t t'. *)
-
-Fixpoint DualT (t t':protoType) : Prop :=
+Definition getP1Type (t:type):type :=
   match t with
-  | Send p1T p1' =>
-    match t' with
-    | Receive p2T p2' => (p1T = p2T) /\ (DualT p1' p2')
-    | _ => False
-    end
-  | Receive p1T p1' =>
-    match t' with
-    | Send p2T p2' => (p1T = p2T) /\ (DualT p1' p2')
-    | _ => False
-    end
-  | Choice p1' p1'' =>
-    match t' with
-    | Offer p2' p2'' => (DualT p1' p2') /\ (DualT p1'' p2'')
-    | _ => False
-    end
-  | Offer p1' p1'' =>
-    match t' with
-    | Choice p2' p2'' => (DualT p1' p2') /\ (DualT p1'' p2'')
-    | _ => False
-    end
-  | Eps _ =>
-    match t' with
-    | Eps _ => True
-    | _ => False
-    end
+  | Pair t1 t2 => t1
+  | _ => t
   end.
 
-Fixpoint DualT_dec (t t':protoType) : {DualT t t'} + {~ DualT t t'}. destruct t. destruct t'. apply right. simpl. unfold not. trivial. assert ({t = t1} + {t <> t1}). apply (eq_type_dec t t1). assert ({DualT t0 t'} + {~ DualT t0 t'}). apply (DualT_dec t0 t'). destruct H. destruct H0. apply left. simpl. split; assumption. apply right. simpl. unfold not. intros. destruct H. contradiction. apply right. unfold not. intros. destruct H. contradiction. right. unfold not. intros. inversion H. right. unfold not. intros. inversion H. right. unfold not. intros. inversion H. destruct t'. assert ({t = t1} + {t <> t1}). apply (eq_type_dec t t1). assert ({DualT t0 t'} + {~ DualT t0 t'}). apply (DualT_dec t0 t'). destruct H. destruct H0. apply left. simpl. split. assumption. assumption. right. unfold not. intros. destruct H. contradiction. apply right. unfold not. intros. destruct H. contradiction. right. unfold not. intros. inversion H. apply right. unfold not. intros. inversion H. apply right. unfold not. intros. inversion H. apply right. unfold not. intros. inversion H. destruct t'. apply right. unfold not. intros. inversion H. apply right. unfold not. intros. inversion H. apply right. unfold not. intros. inversion H. assert ({DualT t1 t'1} + {~ DualT t1 t'1}). apply (DualT_dec t1 t'1). assert ({DualT t2 t'2} + {~ DualT t2 t'2}). apply (DualT_dec t2 t'2). destruct H. destruct H0. left. simpl. split. assumption. assumption. right. unfold not. intros. destruct H. contradiction. right. unfold not. intros. destruct H. contradiction. right. unfold not. intros. inversion H. destruct t'. right. unfold not. intros. inversion H.  right. unfold not. intros. inversion H. assert ({DualT t1 t'1} + {~ DualT t1 t'1}). apply (DualT_dec t1 t'1). assert ({DualT t2 t'2} + {~ DualT t2 t'2}). apply (DualT_dec t2 t'2). destruct H. destruct H0. left. simpl. split; assumption. right. unfold not. intros. destruct H. contradiction. right. unfold not. intros. destruct H. contradiction. right. unfold not. intros. inversion H. right. unfold not. intros. inversion H. destruct t'. right. unfold not. intros. inversion H. right. unfold not. intros. inversion H. right. unfold not. intros. inversion H. right. unfold not. intros. inversion H. left. simpl. trivial. Defined.
+Definition getP2Type (t:type):type :=
+  match t with
+  | Pair t1 t2 => t2
+  | _ => t
+  end.
 
-Definition Dual {t t':protoType} {T T':type} (p1:protoExp T t) (p2:protoExp T' t') : Prop := DualT t t'.
+Definition pairFst{t1 t2: type} (m:message (Pair t1 t2)) : message t1 :=
+  match m in message t' return message (getP1Type t') with 
+  | pair _ _ m1 _ => m1
+  | bad _ => bad _ (*(getP1Type tb1) *)
+  | _ => bad _                
+  end.
+
+Definition pair1 := pair _ _ (basic 1) (basic 2).
+Eval compute in pairFst pair1.
+Definition pair1' := pair _ _ (bad Basic) (basic 2).
+Eval compute in pairFst pair1'.
+Definition pair1'' := pair _ _ (basic 1) (bad Basic).
+Eval compute in pairFst pair1''.
+
+Definition pairSnd{t1 t2: type} (m:message (Pair t1 t2)) : message t2 :=
+  match m in message t' return message (getP2Type t') with
+  | pair _ _ _ m2 => m2
+  | bad _ => bad _ (*(getP1Type tb1) *)
+  | _ => bad _                
+  end.
+
+Definition pair2 := pair _ _ (basic 1) (basic 2).
+Eval compute in pairSnd pair2.
+Definition pair2' := pair _ _ (basic 1) (bad Basic).
+Eval compute in pairSnd pair2'.
 
 Fixpoint protoTypeLength (t:protoType) : nat :=
   match t with
   | Send _ t' => 1 + (protoTypeLength t')
   | Receive _ t' => 1 + (protoTypeLength t')
-  | Choice p1 p2 => protoTypeLength p1
-  | Offer p1 p2 => protoTypeLength p1
-  | Eps _ => 1                                
+  | Choice p1 p2 => 1 + protoTypeLength p2
+  | Offer p1 p2 => 1 + protoTypeLength p2
+  | Eps _ => 1                               
   end.
 
 Definition protoLength {t:protoType} {T:type} (p1:protoExp T t) : nat := protoTypeLength t.
 
 Eval compute in protoTypeLength (Send Basic (Eps Basic)).
 
+Fixpoint DualT' (t t':protoType) : Prop :=
+  match t with
+  | Send p1T p1' =>
+    match t' with
+    | Receive p2T p2' => (p1T = p2T) /\ (DualT' p1' p2')    
+    | _ => False
+    end
+  | Receive p1T p1' =>
+    match t' with
+    | Send p2T p2' => (p1T = p2T) /\ (DualT' p1' p2')                                
+    | _ => False
+    end
+  | Choice p1' p1'' =>
+    match t' with
+    | Offer p2' p2'' => (DualT' p1' p2') /\ (DualT' p1'' p2'')                                                             
+    | _ => False
+    end
+  | Offer p1' p1'' =>
+    match t' with
+    | Choice p2' p2'' => (DualT' p1' p2') /\ (DualT' p1'' p2'')                                                               
+    | _ => False
+    end
+  | Eps _ =>
+    match t' with
+    | Eps _ => True           
+    | _ => False
+    end
+  end.
+
+Definition DualT (t t':protoType) : Prop := DualT' t t'.
+
+Fixpoint DualT_dec (t t':protoType) : {DualT t t'} + {~ DualT t t'}. destruct t. destruct t'. right. simpl. unfold not. trivial. assert ({t = t2} + {t <> t2}). apply (eq_type_dec t t2). assert ({DualT t0 t'} + {~ DualT t0 t'}). apply (DualT_dec t0 t'). destruct H. destruct H0. apply left. unfold DualT. simpl. split; assumption. fold DualT'. apply right. simpl. unfold not. intros. destruct H. contradiction. apply right. unfold not. intros. destruct H. contradiction. right. unfold not. intros. inversion H. right. unfold not. intros. inversion H. right. unfold not. intros. inversion H.
+                                                                     destruct t'. assert ({t = t2} + {t <> t2}). apply (eq_type_dec t t2). assert ({DualT t0 t'} + {~ DualT t0 t'}). apply (DualT_dec t0 t'). destruct H. destruct H0. apply left. simpl. split; assumption.  right. unfold not. intros. destruct H. contradiction. apply right. unfold not. intros. destruct H. contradiction. right. unfold not. intros. inversion H. apply right. unfold not. intros. inversion H. apply right. unfold not. intros. inversion H. apply right. unfold not. intros. inversion H. destruct t'. right. unfold not. intros. inversion H. intros. right. unfold not. intros. inversion H. right. unfold not. intros. inversion H. assert ({DualT t2 t'1 } + {~ DualT t2 t'1}). apply (DualT_dec t2 t'1). assert ({DualT t3 t'2} + {~ DualT t3 t'2}). apply (DualT_dec t3 t'2). destruct H. destruct H0. left. unfold DualT. simpl. split. unfold DualT in d.  unfold DualT in d0. assumption. assumption. right. unfold not. intros. destruct H. contradiction. right. unfold not. intros. destruct H. contradiction. right. unfold not. intros. inversion H.  destruct t'. right. unfold not. intros. inversion H. right. unfold not. intros. inversion H. assert ({DualT t2 t'1} + {~ DualT t2 t'1}). apply (DualT_dec t2 t'1). assert ({DualT t3 t'2} + {~ DualT t3 t'2}). apply (DualT_dec t3 t'2). destruct H. destruct H0. left. simpl. split; assumption. right. unfold not. intros. destruct H. contradiction. right. unfold not. intros. destruct H. contradiction. right. unfold not. intros. inversion H. right. unfold not. intros. inversion H. destruct t'. right. unfold not. intros. inversion H. right. unfold not. intros. inversion H. right. unfold not. intros. inversion H. right. unfold not. intros. inversion H. left. simpl. trivial. Defined.
+
+Definition Dual {t t':protoType} {T T':type} (p1:protoExp T t) (p2:protoExp T' t') : Prop := DualT t t'.            
+
+
 Fixpoint runProto' {t t':protoType} {T T':type} (p1:protoExp T t) (p2:protoExp T' t') (l: nat)
   : (message T) + {(~ (Dual p1 p2))}.
-                    case_eq p1. case_eq p2. intros. apply inright. unfold DualT. unfold not. trivial. intros. assert ({t0 = t1} + {t0 <> t1}). apply (eq_type_dec t0 t1). destruct H1. subst. clear H. clear H0. assert (message T1 + {~ Dual p0 (p m)}). apply (runProto' p'0 p' T1 T0 p0 (p m) (protoTypeLength p'0)). destruct X. apply inleft. exact m0. apply inright. intros. unfold Dual. simpl. unfold Dual in n. unfold not in n. unfold not.  intros. destruct H.  apply n in H0.  assumption. apply inright. unfold Dual. simpl. unfold not. unfold not in n. intros. destruct H1. symmetry in H1. apply n in H1.  assumption. intros. apply inright. unfold Dual. simpl. unfold not. trivial. intros. apply inright. unfold Dual. unfold not. trivial. intros. apply inright. unfold Dual. unfold not. trivial. destruct p2. intros. assert ({t0 = t1} + {t0 <> t1}). apply (eq_type_dec t0 t1). destruct H0. subst. assert (message T1 + {~ Dual (p m) p2 }). apply (runProto' p'0 p' T1 T0 (p m) p2 (protoTypeLength p'0)). destruct X. apply inleft. exact m0. apply inright. intros. unfold Dual. simpl. unfold Dual in n. unfold not in n. unfold not.  intros. destruct H0.  apply n in H1.  assumption. apply inright. unfold Dual. simpl. unfold not. unfold not in n. intros. destruct H0. symmetry in H0. apply n in H0.  assumption. intros. apply inright. unfold Dual. unfold not. trivial. intros.  apply inright. intros. unfold not. intros. inversion H0. intros. apply inright. unfold not. intros. inversion H0. intros. apply inright. unfold not. intros. inversion H0.  intros. destruct p2. destruct b. apply inright. unfold not. intros. inversion H0. apply inright. unfold not. intros. inversion H0. apply inright. unfold not. intros. inversion H0. apply inright. unfold not. intros. inversion H0. destruct b. 
+                    case_eq p1. case_eq p2. intros. apply inright. unfold DualT. unfold not. trivial. intros. assert ({t0 = t2} + {t0 <> t2}). apply (eq_type_dec t0 t2). destruct H1. subst. clear H. clear H0. assert (message T1 + {~ Dual p0 (p m)}). apply (runProto' p'0 p' T1 T0 p0 (p m) (protoTypeLength p'0)). destruct X. apply inleft. exact m0. apply inright. intros. unfold Dual. simpl. unfold Dual in n. unfold not in n. unfold not.  intros. destruct H.  apply n in H0.  assumption. apply inright. unfold Dual. simpl. unfold not. unfold not in n. intros. destruct H1. symmetry in H1. apply n in H1.  assumption. intros. apply inright. unfold Dual. simpl. unfold not. trivial. intros. apply inright. unfold Dual. unfold not. trivial. intros. apply inright. unfold Dual. unfold not. trivial. destruct p2. intros. assert ({t0 = t2} + {t0 <> t2}). apply (eq_type_dec t0 t2). destruct H0. subst. assert (message T1 + {~ Dual (p m) p2 }). apply (runProto' p'0 p' T1 T0 (p m) p2 (protoTypeLength p'0)). destruct X. apply inleft. exact m0. apply inright. intros. unfold Dual. simpl. unfold Dual in n. unfold not in n. unfold not.  intros. destruct H0.  apply n in H1.  assumption. apply inright. unfold Dual. simpl. unfold not. unfold not in n. intros. destruct H0. symmetry in H0. apply n in H0.  assumption. intros. apply inright. unfold Dual. unfold not. trivial. intros.  apply inright. intros. unfold not. intros. inversion H0. intros. apply inright. unfold not. intros. inversion H0. intros. apply inright. unfold not. intros. inversion H0.  intros. destruct p2. destruct b. apply inright. unfold not. intros. inversion H0. apply inright. unfold not. intros. inversion H0. apply inright. unfold not. intros. inversion H0. apply inright. unfold not. intros. inversion H0. destruct b.
 
                     unfold Dual. assert ({DualT r r0} + {~ DualT r r0}). apply (DualT_dec r r0). assert ({DualT s s0} + {~ DualT s s0}). apply (DualT_dec s s0). destruct H0. destruct H1. destruct (runProto' r r0 R R0 p p2_1 (protoTypeLength r0)). left. exact m. unfold not in n. unfold Dual in n. apply n in d. inversion d. right. unfold not. intros. destruct H0. contradiction. right. unfold not. intros. destruct H0. contradiction.
 
-                    unfold Dual. assert ({DualT s s0} + {~ DualT s s0}). apply (DualT_dec s s0). assert ({DualT r r0} + {~ DualT r r0}). apply (DualT_dec r r0). destruct H0. destruct H1. destruct (runProto' s s0 S S0 p0 p2_2 (protoTypeLength s0)). left. exact m. unfold not in n. unfold Dual in n. apply n in d. inversion d. right. unfold not. intros. destruct H0. contradiction. right. unfold not. intros. destruct H0. contradiction. apply inright. intros. unfold not. intros. inversion H0. intros.  
+                    unfold Dual. assert ({DualT s s0} + {~ DualT s s0}). apply (DualT_dec s s0). assert ({DualT r r0} + {~ DualT r r0}). apply (DualT_dec r r0). destruct H0. destruct H1. destruct (runProto' s s0 S S0 p0 p2_2 (protoTypeLength s0)). left. exact m. unfold not in n. unfold Dual in n. apply n in d. inversion d. right. unfold not. intros. destruct H0. contradiction. right. unfold not. intros. destruct H0. contradiction. apply inright. intros. unfold not. intros. inversion H0. intros.
 
                     destruct p2. right. unfold not. intros. inversion H0. right. unfold not. intros. inversion H0. destruct b. unfold Dual. assert ({DualT r r0} + {~ DualT r r0}). apply (DualT_dec r r0). assert ({DualT s s0} + {~ DualT s s0}). apply (DualT_dec s s0). destruct H0. destruct H1. destruct (runProto' s s0 S S0 p0 p2_2 (protoTypeLength s0)). left. exact (reither R S m). unfold not in n. unfold Dual in n. apply n in d0. inversion d0. right. unfold not. intros. destruct H0. contradiction. right. unfold not. intros. destruct H0. contradiction. unfold Dual. assert ({DualT r r0} + {~ DualT r r0}). apply (DualT_dec r r0). assert ({DualT s s0} + {~ DualT s s0}). apply (DualT_dec s s0). destruct H0. destruct H1. destruct (runProto' r r0 R R0 p p2_1 (protoTypeLength r0)). left. exact (leither R S m). unfold not in n. unfold Dual in n. apply n in d. inversion d. right. unfold not. intros. destruct H0. contradiction. right. unfold not. intros. destruct H0. contradiction. right. unfold not. intros. inversion H0. right. unfold not. intros. inversion H0. intros. destruct p2. right. unfold not. intros. inversion H0. right. unfold not. intros. inversion H0. right. unfold not. intros. inversion H0. right. unfold not. intros. inversion H0. left. exact m. Defined.
 
-Inductive protoError {t t':protoType} {T T':type} (p1:protoExp T t) (p2:protoExp T' t') : Type :=
-| NotDual : (~ Dual p1 p2) -> protoError p1 p2
-| NoDecrypt : protoError p1 p2.
   
 Definition runProto {t t':protoType} {T T':type} (p1:protoExp T t) (p2:protoExp T' t')
-  : (message T) + {(~ (Dual p1 p2))} := runProto' p1 p2 (protoLength p1).
+  : (message T) + {(~ (Dual p1 p2))} := runProto' p1 p2 (max (protoLength p1) (protoLength p2)).
 
 Definition proto3 :=
-  send (basic 1);
-  ReturnC (t:=Basic) (basic 1).
+  send (basic 42);
+  ReturnC (t:=Basic) (basic 1). Check proto3.
 
 Definition proto3' :=
   x <- receive;
-  ReturnC (t:=Basic) x.
+  ReturnC (t:=Basic) x. Check proto3'.
+
+Eval compute in (runProto proto3' proto3).
 
 Definition incPayload (m:message Basic) : (message Basic) :=
   match m with
   | basic n => basic (n + 1)
+  | _ => basic 0                 
   end.
   
 Definition proto4 :=
@@ -1117,35 +197,63 @@ Definition proto4 :=
 Check proto4.
 
 Definition proto5 :=
-  send (basic 1);
+  send (basic 42);
   x <- receive;
   ReturnC (t:=Basic) x.
 Check proto5.
 
-Example dual45 : Dual proto4 proto5. unfold Dual. simpl. auto.
+Example dual45 : Dual proto4 proto5. unfold Dual. simpl. auto. Qed.
 
-Definition proto6 :=
-  choice true EpsC
-         proto4. Check proto6.
+Eval compute in (runProto proto5 proto4).
+Eval compute in (runProto proto4 proto5).
+
+Definition proto6 (b:bool) :=
+  choice b EpsC
+         proto5. Check proto6.
 
 Definition proto7 :=
   offer EpsC
-        proto5. Check proto7.
+        proto4. Check proto7.
 
-Example dual67 : Dual proto6 proto7. unfold Dual. simpl. auto. Qed.
-           
-Eval compute in (runProto proto3 proto3').
+Example dual67 : Dual (proto6 false) proto7. unfold Dual. simpl. auto. Qed.
 
-Eval compute in (runProto proto4 proto5).
-Eval compute in (runProto proto5 proto4).
+Eval compute in (runProto (proto6 false) proto7).
+Eval compute in (runProto (proto6 true) proto7).
+
 Eval compute in (runProto proto5 proto3).
-Eval compute in (runProto proto6 proto7).
+
+
+
+Definition aPub := (public 1).
+Definition bPub := (public 2).
+Definition aPubBad := (public 3).
+Definition bPubBad := (public 4).
+Definition aPri := (private 1).
+Definition aPriBad := (private 5).
+Definition bPri := (private 2).
 
 Definition Needham_A :=
-  send (encrypt (Pair Basic Basic) (pair Basic Basic (basic 1) (basic 1))
-                (public 2));
+  send (encrypt Basic (basic 1) bPub);
   x <- receive;
-  send 
-  EpsC.
+  (*y <- decrypt x using aPri; *)
+  send (encrypt _ (pairSnd (t1:=Basic) (t2:=Basic)
+                  (decryptM x aPri)) bPub);
+  ReturnC ((pairSnd (t1:=Basic) (t2:=Basic)
+                  (decryptM x aPri))). Check Needham_A.
 
-End try9.
+Definition Needham_B :=
+  x <- receive;
+  (*y <- decrypt x using bPri; *)
+  send (encrypt _ (pair Basic Basic (decryptM x bPri) (basic 2)) aPub);
+  z <- receive;
+  ReturnC (t:= Pair Basic (Encrypt Basic)) (pair _ _ (decryptM x bPri) z). Check Needham_B.
+
+Example DualNeedham : Dual Needham_A Needham_B.
+Proof. unfold Dual; simpl. repeat( split;trivial). Qed.
+
+Eval compute in runProto Needham_A Needham_B.
+Eval compute in runProto Needham_B Needham_A.
+       
+
+
+End session.
