SessionV2.v
@@ -3,7 +3,7 @@ Require Export CpdtTactics.
 Require Export Crypto.
 
 Module try10.
-
+(*
 Inductive protoType : Type :=
 | Send : type -> protoType -> protoType
 | Receive : type -> protoType -> protoType
@@ -45,10 +45,10 @@ Notation "x :&: y" := (Offer x y)
 Notation "x :&: y" := (protoExp (Offer x y))
                         (at level 50, left associativity).
 
-(*Notation "'send' n ; p" := (SendC n p)
+Notation "'send' n ; p" := (SendC n p)
                             (right associativity, at level 60).
 Notation "x <- 'receive' ; p " := (ReceiveC (fun x => p)) 
-                                    (right associativity, at level 60). *)
+                                    (right associativity, at level 60). 
 
 Notation "'offer'" := OfferC.
 
@@ -139,7 +139,7 @@ Definition incPayload (m:message Basic) : (message Basic) :=
   | basic n => basic (n + 1)
   end.
   
-(*Definition proto4 :=
+Definition proto4 :=
   x <- receive;
   send (incPayload x);
   ReturnC x.
@@ -149,10 +149,10 @@ Definition proto5 :=
   send (basic 1);
   x <- receive;
   ReturnC (t:=Basic) x.
-Check proto5. *)
+Check proto5. 
 
-(*Hint Constructors DualT.
-Example dual45 : Dual proto4 proto5. unfold Dual. auto. Qed.
+
+Example dual45 : Dual proto4 proto5. unfold Dual. simpl. repeat (split; trivial).
 
 Definition proto6 :=
   choice true EpsC
@@ -162,22 +162,11 @@ Definition proto7 :=
   offer EpsC
         proto5. Check proto7.
 
-Example dual67 : Dual proto6 proto7. unfold Dual. auto. Qed.
+Example dual67 : Dual proto6 proto7. unfold Dual. simpl. repeat (split; trivial).
 
 Eval compute in eq_type_dec Basic Basic.
 
 Hint Resolve eq_type_dec.
-
-Example dual45OneStep : DualOneStep proto4 proto5. unfold DualOneStep. reflexivity. Qed.
-
-Example dual67OneStep : DualOneStep proto6 proto7. unfold DualOneStep. reflexivity. Qed.
-
-
-
-Theorem sendsend t t' t0 t1 : (DualT (Send t t0) (Send t' t1)) -> False.
-Proof.
-  intros. inversion H.
-  Qed. 
 
 Fixpoint protoTypeLength (t:protoType) : nat :=
   match t with
@@ -272,7 +261,7 @@ Eval compute in (runProto proto3 proto3' 10).
 End try10.
 
 Module try11.
-
+(*
 Inductive protoType : Type :=
 | Send : type -> protoType -> protoType
 | Receive : type -> protoType -> protoType
@@ -293,7 +282,7 @@ Inductive protoExp : type -> protoType -> Type :=
   : (protoExp R r) -> (protoExp S s) -> (protoExp (if(b) then R else S) (Choice r s))
 | OfferC {r s : protoType} {R S:type}
   : (protoExp R r) -> (protoExp S s) -> (protoExp (Either R S) (Offer r s))
-| DecryptC {p':protoType} {mt T:type} : (message (Encrypt mt)) -> keyType -> ((message mt) -> protoExp T p') -> protoExp T (Decrypt p')   
+| DecryptC {p':protoType} {mt T:type} : (message (Encrypt mt)) -> keyType -> ((message mt) -> protoExp T p') -> protoExp T (Decrypt p')
 | ReturnC {t:type} : (message t) -> protoExp t (Eps t).
 
 Notation "x :!: y" := (Send x y)
@@ -696,7 +685,609 @@ Eval compute in (runProto proto5 proto3).
 Eval compute in (runProto proto6 proto7). *)
 
 
-
+*)
 End try11.
 
 
+Module try12.
+
+Inductive protoType : Type :=
+| Send : type -> protoType -> protoType
+| Receive : type -> protoType -> protoType
+| Choice : protoType -> protoType -> protoType
+| Offer : protoType -> protoType -> protoType  
+| Eps : type -> protoType.
+
+
+Definition t1 := Send (Basic) (Eps Basic). Check t1.
+  
+Inductive protoExp : type -> protoType -> Type :=
+| SendC {t:type} {T:type} {p':protoType}  : (message t) -> (protoExp T p')
+    -> protoExp T (Send t p')
+| ReceiveC {t:type} {T:type} {p':protoType} : ((message t)->(protoExp T p'))     -> protoExp T  (Receive t p') 
+| ChoiceC (b:bool) {r s:protoType} {R S:type} :(protoExp R r) -> (protoExp S s)
+    -> (protoExp (if(b) then R else S) (Choice r s))
+| OfferC {r s : protoType} {R S:type} : (protoExp R r) -> (protoExp S s)
+    -> (protoExp (Either R S) (Offer r s))  
+| ReturnC {t:type} : (message t) -> protoExp t (Eps t).
+
+Notation "x :!: y" := (Send x y)
+                        (at level 50, left associativity). 
+Notation "x :!: y" := (protoExp (Send x y))
+                        (at level 50, left associativity).
+
+Notation "x :?: y" := (Receive x y)
+                        (at level 50, left associativity).  
+Notation "x :?: y" := (protoExp (Receive x y))
+                        (at level 50, left associativity).
+
+Notation "x :+: y" := (Choice x y)
+                        (at level 50, left associativity).
+Notation "x :+: y" := (protoExp (Choice x y))
+                        (at level 50, left associativity). 
+
+Notation "x :&: y" := (Offer x y)
+                        (at level 50, left associativity).
+Notation "x :&: y" := (protoExp (Offer x y))
+                        (at level 50, left associativity).
+
+Notation "'send' n ; p" := (SendC n p)
+                            (right associativity, at level 60).
+Notation "x <- 'receive' ; p " := (ReceiveC (fun x => p)) 
+                                    (right associativity, at level 60).
+
+Notation "'offer'" := OfferC.
+
+Notation "'choice'" := ChoiceC.
+
+Definition EpsC := ReturnC (basic 0).
+Definition proto1 := SendC (basic 1) EpsC.
+Check proto1.
+
+Definition unwrapBasic (m:message Basic) : nat :=
+  match m with
+  | basic n => n
+  | _ => 0
+  end.
+
+
+Definition enc1 := encrypt Basic (basic 42) (public 1). Check enc1.
+Definition enc2 := encrypt _ enc1 (public 2).
+Eval compute in decryptM enc1 (private 1).
+Eval compute in decryptM enc1 (private 0).
+Eval compute in decryptM enc2 (private 2).
+Eval compute in decryptM (decryptM enc2 (private 2)) (private 1).
+
+Definition getP1Type (t:type):type :=
+  match t with
+  | Pair t1 t2 => t1
+  | _ => t
+  end.
+
+Definition getP2Type (t:type):type :=
+  match t with
+  | Pair t1 t2 => t2
+  | _ => t
+  end.
+
+Definition pairFst{t1 t2: type} (m:message (Pair t1 t2)) : message t1 :=
+  match m in message t' return message (getP1Type t') with 
+  | pair _ _ m1 _ => m1
+  | bad _ => bad _ (*(getP1Type tb1) *)
+  | _ => bad _                
+  end.
+
+Definition pair1 := pair _ _ (basic 1) (basic 2).
+Eval compute in pairFst pair1.
+Definition pair1' := pair _ _ (bad Basic) (basic 2).
+Eval compute in pairFst pair1'.
+Definition pair1'' := pair _ _ (basic 1) (bad Basic).
+Eval compute in pairFst pair1''.
+
+Definition pairSnd{t1 t2: type} (m:message (Pair t1 t2)) : message t2 :=
+  match m in message t' return message (getP2Type t') with
+  | pair _ _ _ m2 => m2
+  | bad _ => bad _ (*(getP1Type tb1) *)
+  | _ => bad _                
+  end.
+
+Definition pair2 := pair _ _ (basic 1) (basic 2).
+Eval compute in pairSnd pair2.
+Definition pair2' := pair _ _ (basic 1) (bad Basic).
+Eval compute in pairSnd pair2'.
+
+Fixpoint protoTypeLength (t:protoType) : nat :=
+  match t with
+  | Send _ t' => 1 + (protoTypeLength t')
+  | Receive _ t' => 1 + (protoTypeLength t')
+  | Choice p1 p2 => 1 + protoTypeLength p2
+  | Offer p1 p2 => 1 + protoTypeLength p2
+  | Eps _ => 1                               
+  end.
+
+Definition protoLength {t:protoType} {T:type} (p1:protoExp T t) : nat := protoTypeLength t.
+
+Eval compute in protoTypeLength (Send Basic (Eps Basic)).
+
+Fixpoint DualT' (t t':protoType) : Prop :=
+  match t with
+  | Send p1T p1' =>
+    match t' with
+    | Receive p2T p2' => (p1T = p2T) /\ (DualT' p1' p2')    
+    | _ => False
+    end
+  | Receive p1T p1' =>
+    match t' with
+    | Send p2T p2' => (p1T = p2T) /\ (DualT' p1' p2')                                
+    | _ => False
+    end
+  | Choice p1' p1'' =>
+    match t' with
+    | Offer p2' p2'' => (DualT' p1' p2') /\ (DualT' p1'' p2'')                                                             
+    | _ => False
+    end
+  | Offer p1' p1'' =>
+    match t' with
+    | Choice p2' p2'' => (DualT' p1' p2') /\ (DualT' p1'' p2'')                                                               
+    | _ => False
+    end
+  | Eps _ =>
+    match t' with
+    | Eps _ => True           
+    | _ => False
+    end
+  end.
+
+Definition DualT (t t':protoType) : Prop := DualT' t t'.
+
+Fixpoint DualT_dec (t t':protoType) : {DualT t t'} + {~ DualT t t'}. destruct t. destruct t'. right. simpl. unfold not. trivial. assert ({t = t2} + {t <> t2}). apply (eq_type_dec t t2). assert ({DualT t0 t'} + {~ DualT t0 t'}). apply (DualT_dec t0 t'). destruct H. destruct H0. apply left. unfold DualT. simpl. split; assumption. fold DualT'. apply right. simpl. unfold not. intros. destruct H. contradiction. apply right. unfold not. intros. destruct H. contradiction. right. unfold not. intros. inversion H. right. unfold not. intros. inversion H. right. unfold not. intros. inversion H.
+                                                                     destruct t'. assert ({t = t2} + {t <> t2}). apply (eq_type_dec t t2). assert ({DualT t0 t'} + {~ DualT t0 t'}). apply (DualT_dec t0 t'). destruct H. destruct H0. apply left. simpl. split; assumption.  right. unfold not. intros. destruct H. contradiction. apply right. unfold not. intros. destruct H. contradiction. right. unfold not. intros. inversion H. apply right. unfold not. intros. inversion H. apply right. unfold not. intros. inversion H. apply right. unfold not. intros. inversion H. destruct t'. right. unfold not. intros. inversion H. intros. right. unfold not. intros. inversion H. right. unfold not. intros. inversion H. assert ({DualT t2 t'1 } + {~ DualT t2 t'1}). apply (DualT_dec t2 t'1). assert ({DualT t3 t'2} + {~ DualT t3 t'2}). apply (DualT_dec t3 t'2). destruct H. destruct H0. left. unfold DualT. simpl. split. unfold DualT in d.  unfold DualT in d0. assumption. assumption. right. unfold not. intros. destruct H. contradiction. right. unfold not. intros. destruct H. contradiction. right. unfold not. intros. inversion H.  destruct t'. right. unfold not. intros. inversion H. right. unfold not. intros. inversion H. assert ({DualT t2 t'1} + {~ DualT t2 t'1}). apply (DualT_dec t2 t'1). assert ({DualT t3 t'2} + {~ DualT t3 t'2}). apply (DualT_dec t3 t'2). destruct H. destruct H0. left. simpl. split; assumption. right. unfold not. intros. destruct H. contradiction. right. unfold not. intros. destruct H. contradiction. right. unfold not. intros. inversion H. right. unfold not. intros. inversion H. destruct t'. right. unfold not. intros. inversion H. right. unfold not. intros. inversion H. right. unfold not. intros. inversion H. right. unfold not. intros. inversion H. left. simpl. trivial. Defined.
+
+Definition Dual {t t':protoType} {T T':type} (p1:protoExp T t) (p2:protoExp T' t') : Prop := DualT t t'.            
+
+
+Fixpoint runProto' {t t':protoType} {T T':type} (p1:protoExp T t) (p2:protoExp T' t') (l: nat)
+  : (message T) + {(~ (Dual p1 p2))}.
+                    case_eq p1. case_eq p2. intros. apply inright. unfold DualT. unfold not. trivial. intros. assert ({t0 = t2} + {t0 <> t2}). apply (eq_type_dec t0 t2). destruct H1. subst. clear H. clear H0. assert (message T1 + {~ Dual p0 (p m)}). apply (runProto' p'0 p' T1 T0 p0 (p m) (protoTypeLength p'0)). destruct X. apply inleft. exact m0. apply inright. intros. unfold Dual. simpl. unfold Dual in n. unfold not in n. unfold not.  intros. destruct H.  apply n in H0.  assumption. apply inright. unfold Dual. simpl. unfold not. unfold not in n. intros. destruct H1. symmetry in H1. apply n in H1.  assumption. intros. apply inright. unfold Dual. simpl. unfold not. trivial. intros. apply inright. unfold Dual. unfold not. trivial. intros. apply inright. unfold Dual. unfold not. trivial. destruct p2. intros. assert ({t0 = t2} + {t0 <> t2}). apply (eq_type_dec t0 t2). destruct H0. subst. assert (message T1 + {~ Dual (p m) p2 }). apply (runProto' p'0 p' T1 T0 (p m) p2 (protoTypeLength p'0)). destruct X. apply inleft. exact m0. apply inright. intros. unfold Dual. simpl. unfold Dual in n. unfold not in n. unfold not.  intros. destruct H0.  apply n in H1.  assumption. apply inright. unfold Dual. simpl. unfold not. unfold not in n. intros. destruct H0. symmetry in H0. apply n in H0.  assumption. intros. apply inright. unfold Dual. unfold not. trivial. intros.  apply inright. intros. unfold not. intros. inversion H0. intros. apply inright. unfold not. intros. inversion H0. intros. apply inright. unfold not. intros. inversion H0.  intros. destruct p2. destruct b. apply inright. unfold not. intros. inversion H0. apply inright. unfold not. intros. inversion H0. apply inright. unfold not. intros. inversion H0. apply inright. unfold not. intros. inversion H0. destruct b.
+
+                    unfold Dual. assert ({DualT r r0} + {~ DualT r r0}). apply (DualT_dec r r0). assert ({DualT s s0} + {~ DualT s s0}). apply (DualT_dec s s0). destruct H0. destruct H1. destruct (runProto' r r0 R R0 p p2_1 (protoTypeLength r0)). left. exact m. unfold not in n. unfold Dual in n. apply n in d. inversion d. right. unfold not. intros. destruct H0. contradiction. right. unfold not. intros. destruct H0. contradiction.
+
+                    unfold Dual. assert ({DualT s s0} + {~ DualT s s0}). apply (DualT_dec s s0). assert ({DualT r r0} + {~ DualT r r0}). apply (DualT_dec r r0). destruct H0. destruct H1. destruct (runProto' s s0 S S0 p0 p2_2 (protoTypeLength s0)). left. exact m. unfold not in n. unfold Dual in n. apply n in d. inversion d. right. unfold not. intros. destruct H0. contradiction. right. unfold not. intros. destruct H0. contradiction. apply inright. intros. unfold not. intros. inversion H0. intros.
+
+                    destruct p2. right. unfold not. intros. inversion H0. right. unfold not. intros. inversion H0. destruct b. unfold Dual. assert ({DualT r r0} + {~ DualT r r0}). apply (DualT_dec r r0). assert ({DualT s s0} + {~ DualT s s0}). apply (DualT_dec s s0). destruct H0. destruct H1. destruct (runProto' s s0 S S0 p0 p2_2 (protoTypeLength s0)). left. exact (reither R S m). unfold not in n. unfold Dual in n. apply n in d0. inversion d0. right. unfold not. intros. destruct H0. contradiction. right. unfold not. intros. destruct H0. contradiction. unfold Dual. assert ({DualT r r0} + {~ DualT r r0}). apply (DualT_dec r r0). assert ({DualT s s0} + {~ DualT s s0}). apply (DualT_dec s s0). destruct H0. destruct H1. destruct (runProto' r r0 R R0 p p2_1 (protoTypeLength r0)). left. exact (leither R S m). unfold not in n. unfold Dual in n. apply n in d. inversion d. right. unfold not. intros. destruct H0. contradiction. right. unfold not. intros. destruct H0. contradiction. right. unfold not. intros. inversion H0. right. unfold not. intros. inversion H0. intros. destruct p2. right. unfold not. intros. inversion H0. right. unfold not. intros. inversion H0. right. unfold not. intros. inversion H0. right. unfold not. intros. inversion H0. left. exact m. Defined.
+
+  
+Definition runProto {t t':protoType} {T T':type} (p1:protoExp T t) (p2:protoExp T' t')
+  : (message T) + {(~ (Dual p1 p2))} := runProto' p1 p2 (max (protoLength p1) (protoLength p2)).
+
+Definition proto3 :=
+  send (basic 42);
+  ReturnC (t:=Basic) (basic 1). Check proto3.
+
+Definition proto3' :=
+  x <- receive;
+  ReturnC (t:=Basic) x. Check proto3'.
+
+Eval compute in (runProto proto3' proto3).
+
+Definition incPayload (m:message Basic) : (message Basic) :=
+  match m with
+  | basic n => basic (n + 1)
+  | _ => basic 0                 
+  end.
+  
+Definition proto4 :=
+  x <- receive;
+  send (incPayload x);
+  ReturnC x.
+Check proto4.
+
+Definition proto5 :=
+  send (basic 42);
+  x <- receive;
+  ReturnC (t:=Basic) x.
+Check proto5.
+
+Example dual45 : Dual proto4 proto5. unfold Dual. simpl. auto. Qed.
+
+Eval compute in (runProto proto5 proto4).
+Eval compute in (runProto proto4 proto5).
+
+Definition proto6 (b:bool) :=
+  choice b EpsC
+         proto5. Check proto6.
+
+Definition proto7 :=
+  offer EpsC
+        proto4. Check proto7.
+
+Example dual67 : Dual (proto6 false) proto7. unfold Dual. simpl. auto. Qed.
+
+Eval compute in (runProto (proto6 false) proto7).
+Eval compute in (runProto (proto6 true) proto7).
+
+Eval compute in (runProto proto5 proto3).
+
+
+
+Definition aPub := (public 1).
+Definition bPub := (public 2).
+Definition aPubBad := (public 3).
+Definition bPubBad := (public 4).
+Definition aPri := (private 1).
+Definition aPriBad := (private 5).
+Definition bPri := (private 2).
+
+Definition Needham_A :=
+  send (encrypt Basic (basic 1) bPub);
+  x <- receive;
+  (*y <- decrypt x using aPri; *)
+  send (encrypt _ (pairSnd (t1:=Basic) (t2:=Basic)
+                  (decryptM x aPri)) bPub);
+  ReturnC ((pairSnd (t1:=Basic) (t2:=Basic)
+                  (decryptM x aPri))). Check Needham_A.
+
+Definition Needham_B :=
+  x <- receive;
+  (*y <- decrypt x using bPri; *)
+  send (encrypt _ (pair Basic Basic (decryptM x bPri) (basic 2)) aPub);
+  z <- receive;
+  ReturnC (t:= Pair Basic (Encrypt Basic)) (pair _ _ (decryptM x bPri) z). Check Needham_B.
+
+Example DualNeedham : Dual Needham_A Needham_B.
+Proof. unfold Dual; simpl. repeat( split;trivial). Qed.
+
+Eval compute in runProto Needham_A Needham_B.
+Eval compute in runProto Needham_B Needham_A.
+       
+
+
+End try12.
+
+
+
+Module try13.
+
+Inductive protoType : Type :=
+| Send : type -> protoType -> protoType
+| Receive : type -> protoType -> protoType
+| Choice : protoType -> protoType -> protoType
+| Offer : protoType -> protoType -> protoType
+(*| Decrypt : protoType -> protoType  *)                                  
+| Eps : type -> protoType.
+
+(*Inductive Either (A:Type) (B:Type) : Type :=
+| eLeft : A -> Either A B
+| eRight : B -> Either A B. *)
+
+  
+Inductive protoExp : type -> protoType -> Type :=
+| SendC {t:type} {T:type} {p':protoType}  : (message t) -> (protoExp T p') -> protoExp T (Send t p')
+| ReceiveC {t:type} {T:type} {p':protoType} : ((message t)->(protoExp T p')) -> protoExp T  (Receive t p') 
+| ChoiceC (b:bool) {r s: protoType} {R S:type}
+  : (protoExp R r) -> (protoExp S s) -> (protoExp (if(b) then R else S) (Choice r s))
+| OfferC {r s : protoType} {R S:type}
+  : (protoExp R r) -> (protoExp S s) -> (protoExp (Either R S) (Offer r s))
+| DecryptC {p':protoType} {mt T:type} : (message (Encrypt mt)) -> keyType -> ((message mt) -> protoExp T p') -> protoExp T p'(*(Decrypt p')*)
+| ReturnC {t:type} : (message t) -> protoExp t (Eps t).
+
+Notation "x :!: y" := (Send x y)
+                        (at level 50, left associativity). 
+Notation "x :!: y" := (protoExp (Send x y))
+                        (at level 50, left associativity).
+
+Notation "x :?: y" := (Receive x y)
+                        (at level 50, left associativity).  
+Notation "x :?: y" := (protoExp (Receive x y))
+                        (at level 50, left associativity).
+
+(*Notation "x :D: y" := (Decrypt x y)
+                        (at level 50, left associativity).  
+Notation "x :D: y" := (protoExp (Decrypt x y))
+                        (at level 50, left associativity). *)
+
+Notation "x :+: y" := (Choice x y)
+                        (at level 50, left associativity).
+Notation "x :+: y" := (protoExp (Choice x y))
+                        (at level 50, left associativity). 
+
+Notation "x :&: y" := (Offer x y)
+                        (at level 50, left associativity).
+Notation "x :&: y" := (protoExp (Offer x y))
+                        (at level 50, left associativity).
+
+Notation "'send' n ; p" := (SendC n p)
+                            (right associativity, at level 60).
+(*Notation "x <- 'receive' ; p " := (ReceiveC (fun x => p)) 
+                                    (right associativity, at level 60). *)
+
+Notation "z <- 'decrypt' m 'using' k ; p " := (DecryptC m k (fun z => p)) 
+                                    (right associativity, at level 60(*, m ident, k ident)*)).
+Notation "'offer'" := OfferC.
+
+Notation "'choice'" := ChoiceC.
+
+Definition EpsC := ReturnC (basic 0).
+Definition proto1 := SendC (basic 1) EpsC.
+Check proto1.
+
+Definition unwrapBasic (m:message Basic) : nat :=
+  match m with
+  | basic n => n
+  end.
+
+Definition unwrapEncrypt {mt:type} (m:message (Encrypt mt)) : message mt :=
+  match m with
+  | encrypt _ m' _ => m'
+  end.
+
+
+Definition enc1 := encrypt Basic (basic 42) (public 1). Check enc1.
+Definition enc2 := encrypt _ enc1 (public 2).
+Eval compute in unwrapEncrypt enc1.
+Eval compute in unwrapEncrypt enc2.
+
+
+Definition proto2 :=
+  SendC (basic 1)
+  ( ReceiveC (fun x =>
+  ( ReceiveC (fun y =>
+  ( DecryptC enc1 (public 1) (fun z =>                            
+  ( SendC (basic ((unwrapBasic x) + (unwrapBasic y)))
+  ( EpsC)))))))).              
+Check proto2.
+Check DecryptC.
+(*Definition proto2D :=
+  send (basic 1);
+  x <- receive;
+  y <- receive;
+  z <- decrypt enc1 using (public 1);                        
+  ( SendC (basic ((unwrapBasic x) + (unwrapBasic y)))
+  ( EpsC)).              
+Check proto2.
+
+Definition dec1 := SendC (basic 1)
+                         (DecryptC enc1 (public 1) (fun x => (ReturnC x))). Check dec1.
+
+Check (public 1).
+
+Definition dec2 := DecryptC enc1 (public 1) (fun x => ReturnC x). Check dec2.
+Definition dec2Proro :=
+  x <- decrypt (enc1) using (public 1) ; ((ReturnC x)).
+
+Definition decryptProto :=
+  send (basic 1);
+  x <- decrypt enc1 using (public 1);
+  send (basic 1); EpsC.
+
+Definition pairFst{t1 t2: type} (m:message (Pair t1 t2)) : message t1 :=
+  match m with
+  | pair _ _ m1 _ => m1
+  end.
+
+Definition pairSnd{t1 t2: type} (m:message (Pair t1 t2)) : message t2 :=
+  match m with
+  | pair _ _ _ m2 => m2
+  end. *)
+
+
+Fixpoint protoTypeLength (t:protoType) : nat :=
+  match t with
+  | Send _ t' => 1 + (protoTypeLength t')
+  | Receive _ t' => 1 + (protoTypeLength t')
+  | Choice p1 p2 => 1 + protoTypeLength p2
+  | Offer p1 p2 => 1 + protoTypeLength p2
+  (*| Decrypt p' => 1 + (protoTypeLength p') *)
+  | Eps _ => 1                               
+  end.
+
+Definition protoLength {t:protoType} {T:type} (p1:protoExp T t) : nat := protoTypeLength t.
+
+Eval compute in protoTypeLength (Send Basic (Eps Basic)).
+
+Fixpoint DualT (t t':protoType) : Prop :=
+  match t with
+  | Send p1T p1' =>
+    match t' with
+    | Receive p2T p2' => (p1T = p2T) /\ (DualT p1' p2')
+    (*| Decrypt t'' => DualT'' t t''      *)     
+    | _ => False
+    end
+  | Receive p1T p1' =>
+    match t' with
+    | Send p2T p2' => (p1T = p2T) /\ (DualT p1' p2')                                
+    | _ => False
+    end
+  | Choice p1' p1'' =>
+    match t' with
+    | Offer p2' p2'' => (DualT p1' p2') /\ (DualT p1'' p2'')                                                             
+    | _ => False
+    end
+  | Offer p1' p1'' =>
+    match t' with
+    | Choice p2' p2'' => (DualT p1' p2') /\ (DualT p1'' p2'')                                                               
+    | _ => False
+    end
+  (*| Decrypt p1' => DualT' p1' t' (*Check this *)  *)
+  | Eps _ =>
+    match t' with
+    | Eps _ => True           
+    | _ => False
+    end
+  end.
+
+Fixpoint DualT_dec (t t':protoType) : {DualT t t'} + {~ DualT t t'}. destruct t. destruct t'. apply right. simpl. unfold not. trivial. assert ({t = t1} + {t <> t1}). apply (eq_type_dec t t1). assert ({DualT t0 t'} + {~ DualT t0 t'}). apply (DualT_dec t0 t'). destruct H. destruct H0. apply left. unfold DualT. simpl. split; assumption. fold DualT; try (apply right; simpl; unfold not; intros; destruct H; contradiction). try (right; unfold not; intros; inversion H). contradiction. right. unfold not. intros. inversion H. right. unfold not. intros. inversion H.
+
+                                                                     right. unfold not. intros. inversion H.  destruct t'. assert ({t = t1} + {t <> t1}). apply (eq_type_dec t t1). assert ({DualT t0 t'} + {~ DualT t0 t'}). apply (DualT_dec t0 t'). destruct H. destruct H0. apply left. simpl. split. assumption. unfold DualT in d. assumption. right. unfold not. intros. destruct H. contradiction. apply right. unfold not. intros. destruct H. contradiction. right. unfold not. intros. inversion H. apply right. unfold not. intros. inversion H. apply right. unfold not. intros. inversion H. apply right. unfold not. intros. inversion H. destruct t'. apply right. unfold not. intros. inversion H. apply right. unfold not. intros. inversion H. apply right. unfold not. intros. inversion H. assert ({DualT t1 t'1 (* (max (protoTypeLength t2) (protoTypeLength t'2))*)} + {~ DualT t1 t'1 (*(max (protoTypeLength t2) (protoTypeLength t'2))*)}). apply (DualT_dec t1 t'1). assert ({DualT t2 t'2} + {~ DualT t2 t'2}). apply (DualT_dec t2 t'2). destruct H. destruct H0. left. unfold DualT. simpl. split. unfold DualT in d.  unfold DualT in d0. assumption. assumption. right. unfold not. intros. destruct H. contradiction. right. unfold not. intros. destruct H. contradiction. right. unfold not. intros. inversion H. destruct t'. right. unfold not. intros. inversion H.  right. unfold not. intros. inversion H. assert ({DualT t1 t'1} + {~ DualT t1 t'1}). apply (DualT_dec t1 t'1). assert ({DualT t2 t'2} + {~ DualT t2 t'2}). apply (DualT_dec t2 t'2). destruct H. destruct H0. left. simpl. split; assumption. right. unfold not. intros. destruct H. contradiction. right. unfold not. intros. destruct H. contradiction. right. unfold not. intros. inversion H. right. unfold not. intros. inversion H. destruct t'. right. unfold not. intros. inversion H. right. unfold not. intros. inversion H. right. unfold not. intros. inversion H. right. unfold not. intros. inversion H. left. simpl. trivial. Defined.
+
+(*Definition isDual := DualT_dec (Decrypt (Eps Basic)) (Eps Basic).
+Eval compute in isDual. *)
+
+Definition Dual {t t':protoType} {T T':type} (p1:protoExp T t) (p2:protoExp T' t') : Prop := DualT t t'.
+
+(*Definition dualProto1 :=
+  send (basic 1);
+  x <- decrypt enc1 using (public 0);
+  y <- receive;
+  ReturnC (t:=Basic) y.
+
+Definition dualProto2 :=
+  x <- receive;
+  send (basic 1);
+  ReturnC (t:=Basic) x.
+
+Example dual12 : Dual dualProto1 dualProto2. unfold Dual. simpl. split. trivial. split; trivial. Qed.
+
+Definition aPub := (public 1).
+Definition bPub := (public 2).
+Definition aPri := (private 1).
+Definition bPri := (private 2).
+
+Definition Needham_A :=
+  send (encrypt Basic (basic 1) bPub);
+  x <- receive;
+  y <- decrypt x using aPri;
+  send (encrypt _ (pairSnd (t1:=Basic) (t2:=Basic) y) (public 2));
+  EpsC. Check Needham_A.
+
+Definition Needham_B :=
+  x <- receive;
+  y <- decrypt x using bPri;
+  send (encrypt (Pair Basic Basic) (pair Basic Basic y (basic 2)) aPub);
+  z <- receive;
+  ReturnC (t:= Encrypt Basic) z. Check Needham_B.
+
+Example DualTNeed : DualT
+(Send (Encrypt Basic) (* (Decrypt ( *)
+  (Receive (Encrypt (Pair Basic Basic))
+    (Send (Encrypt Basic) (Eps Basic)))) (* )) *)
+
+(Receive (Encrypt Basic)
+  (Send (Encrypt (Pair Basic Basic)) (*(Decrypt ( *)
+    (Receive (Encrypt Basic) (Eps (Encrypt Basic)))))(*))*). simpl; try (split; trivial). split; trivial. split; trivial. Qed.
+
+Example DualNeedham : Dual Needham_A Needham_B.
+Proof. unfold Dual. split. trivial. split. trivial. split. trivial. simpl. trivial. Qed.
+
+(*Definition Dual_dec {t t':protoType} {T T':type} (p1:protoExp T t) (p2:protoExp T' t') : {Dual p1 p2} + {~ Dual p1 p2}. assert ({DualT t t'} + {~DualT t t'}). apply (DualT_dec t t'). destruct p1. destruct p2. right. unfold not. intros. inversion H0.
+  refine (
+      match (DualT_dec t t') with
+      | left _ => left _
+      | right _ => right _
+      end                  
+  ). *)
+
+
+*)
+
+Inductive protoError {t t':protoType} {T T':type} (p1:protoExp T t) (p2:protoExp T' t') : Prop :=
+| NotDual : (~Dual p1 p2) -> protoError p1 p2
+| NoDecrypt : (*forall  (m:message t) (k:keyType), (is_not_decryptable t m k) -> *) protoError p1 p2.            
+
+Fixpoint runProto' {t t':protoType} {T T':type} (p1:protoExp T t) (p2:protoExp T' t') (l: nat)
+  : (message T) + {(protoError p1 p2)}. (*{(~ (Dual p1 p2))}*)
+                    case_eq p1. case_eq p2; intros. apply inright. apply NotDual. unfold not. trivial. assert ({t0 = t1} + {t0 <> t1}). apply (eq_type_dec t0 t1). destruct H1. subst. clear H. clear H0. assert (message T1 + {(protoError p0 (p m))}). apply (runProto' p'0 p' T1 T0 p0 (p m) (protoTypeLength p'0)). destruct X. apply inleft. exact m0. apply inright. destruct p3. apply NotDual. unfold not. intros. inversion H0. contradiction. apply NoDecrypt. clear H. clear H0. apply inright. apply NotDual. unfold not. intros. inversion H. symmetry in H0. contradiction. apply inright. apply NotDual. unfold not. intros. inversion H1. intros. apply inright. apply NotDual. unfold not. intros. inversion H1. (*assert ({T0=T1}+{T0<>T1}). apply (eq_type_dec T0 T1). destruct H1. subst.*) destruct (decrypt m k).
+                    assert (message T1 + {(protoError (SendC m0 p0) (p m1))}). apply (runProto' _ _ _ _ (SendC m0 p0) (p m1) (protoTypeLength p'0)). destruct X. apply inleft. exact m2. clear H0. clear H. assert ({DualT (Send t0 p'0) p'}+{~DualT (Send t0 p'0) p'}). apply (DualT_dec (Send t0 p'0) p'). destruct H. apply inright. apply NoDecrypt. apply inright. apply NotDual.
+                    unfold not. intros. unfold Dual in H. contradiction. apply inright. apply NoDecrypt. apply inright. apply NotDual. unfold not. intros. contradiction. intros. destruct p2. assert ({t0 = t1} + {t0 <> t1}). apply (eq_type_dec t0 t1). destruct H0. subst. clear H. assert (message T0 + {(protoError (p m) p2)}). apply (runProto' _ _ _ _ (p m) p2 (protoTypeLength p')). destruct X. apply inleft. exact m0. apply inright. destruct p0. apply NotDual. unfold not. intros. inversion H0. contradiction. apply NoDecrypt. clear H. apply inright. apply NotDual. unfold not. intros. inversion H. contradiction. apply inright. apply NotDual. unfold not. intros. inversion H0. apply inright. apply NotDual. unfold not. intros. inversion H0. apply inright. apply NotDual. unfold not. intros. inversion H0. assert ({(DualT (Receive t0 p') p'0)} + {~(DualT (Receive t0 p') p'0)}). apply (DualT_dec (Receive t0 p') p'0). destruct H0. destruct (decrypt m k). assert ({DualT (Receive t0 p') p'0}+{~DualT (Receive t0 p') p'0}). apply (DualT_dec (Receive t0 p') p'0). destruct H0. apply p0 in m0.
+
+                    assert (message T0 + {(protoError (ReceiveC p) m0)}). apply (runProto' _ _ _ _ (ReceiveC p) m0 (protoTypeLength p'0)). destruct X. apply inleft. exact m1. apply inright. apply NoDecrypt. apply inright. apply NotDual. unfold not. intros. unfold Dual in H0. contradiction. apply inright. apply NoDecrypt. apply inright. apply NotDual. unfold not. intros. unfold Dual in H0. contradiction. apply inright. apply NotDual. unfold not. intros. unfold Dual in H0. contradiction. intros.
+
+                    (*assert ({DualT (Send t0 p'0) p'}+{~DualT (Send t0 p'0) p'}). apply (DualT_dec (Send t0 p'0) p'). destruct H. apply inright. apply NoDecrypt. apply inright. apply NotDual. 
+                    
+n
+                    assert ({T0=T1}+{T0<>T1}). apply (eq_type_dec T0 T1). simpl in d. destruct p'0. destruct d. subst. apply p0 in m0. destruct m0. assert ({t0 = t1} + {t0<>t1}). apply (eq_type_dec t0 t1). destruct H1. subst.
+                    assert (message T0 + {(protoError (p m0) m1)}). apply (runProto' _ _ _ _  (p m0) m1 (protoTypeLength p'0)). destruct X. apply inleft. exact m2. clear H. subst. apply inright. apply NoDecrypt. apply inright. apply NoDecrypt. apply inright. apply NoDecrypt. 
+
+                    apply inright. apply NotDual. unfold not. intros. inversion H0. contradiction. contradiction.  apply inright. apply NotDual. unfold not. intros. contradiction. apply inright. apply NotDual. unfold not. intros. destruct b. destruct p2. apply inright. apply NotDual. unfold not. intros. inversion H0. apply inright. apply NotDual. unfold not. intros. inversion H0. apply inright. apply NotDual. unfold not. intros. inversion H0.
+                    assert ({DualT r r0} + {~ DualT r r0}). apply (DualT_dec r r0). assert ({DualT s s0} + {~ DualT s s0}). apply (DualT_dec s s0). destruct H0. destruct H1. destruct (runProto' r r0 R R0 p p2_1 (protoTypeLength r0)). left. exact m. apply inright. destruct p2. contradiction. apply NoDecrypt. apply inright. apply NotDual. unfold not. intros. inversion H0. contradiction. apply inright. apply NotDual. unfold not. intros. inversion H0. contradiction. apply inright. apply NotDual. unfold not. intros. inversion H0.  apply inright. apply NotDual. unfold not. intros. inversion H0. destruct p2. apply inright. apply NotDual. unfold not. intros. inversion H0. apply inright. apply NotDual. unfold not. intros. inversion H0. apply inright. apply NotDual. unfold not. intros. inversion H0.
+
+                    assert ({DualT r r0} + {~ DualT r r0}). apply (DualT_dec r r0). assert ({DualT s s0} + {~ DualT s s0}). apply (DualT_dec s s0). destruct H0. destruct H1. destruct (runProto' _ _ _ _ p0 p2_2 (protoTypeLength s)). left. exact m. apply inright. destruct p2. contradiction. apply NoDecrypt. apply inright. apply NotDual. unfold not. intros. inversion H0. contradiction. apply inright. apply NotDual. unfold not. intros. inversion H0. contradiction. apply inright. apply NotDual. unfold not. intros. inversion H0.  apply inright. apply NotDual. unfold not. intros. inversion H0. intros. destruct p2. apply inright. apply NotDual. unfold not. intros. inversion H0. apply inright. apply NotDual. unfold not. intros. inversion H0. assert ({DualT r r0} + {~ DualT r r0}). apply (DualT_dec r r0). assert ({DualT s s0} + {~ DualT s s0}). apply (DualT_dec s s0). destruct H0. destruct H1. destruct b. destruct (runProto' _ _ _ _ p p2_1 (protoTypeLength r)). apply inleft. exact (leither _ _ m). apply inright. destruct p2. apply NotDual. unfold not. intros. inversion H1. contradiction. apply NoDecrypt. destruct (runProto' _ _ _ _ p0 p2_2 (protoTypeLength s)). apply inleft. exact (reither _ _ m). apply inright. destruct p2. apply NotDual. unfold not. intros. inversion H1. contradiction. apply NoDecrypt. apply inright. apply NotDual. unfold not. intros. inversion H0. contradiction. apply inright. apply NotDual. unfold not. intros. inversion H0. contradiction. apply inright. apply NotDual. unfold not. intros. inversion H0. apply inright. apply NotDual. unfold not. intros. inversion H0. apply inright. apply NotDual. unfold not. intros. inversion H0. intros. clear H. destruct (is_not_decryptable
+
+                    apply inright. apply NotDual. unfold not. intros. inversion H0.
+
+                    apply NotDual. unfold not in n. unfold Dual in n. apply n in d. inversion d. right. unfold not. intros. destruct H0. contradiction. right. unfold not. intros. destruct H0. contradiction.
+
+                    unfold Dual. assert ({DualT s s0} + {~ DualT s s0}). apply (DualT_dec s s0). assert ({DualT r r0} + {~ DualT r r0}). apply (DualT_dec r r0). destruct H0. destruct H1. destruct (runProto' s s0 S S0 p0 p2_2 (protoTypeLength s0)). left. exact m. unfold not in n. unfold Dual in n. apply n in d. inversion d. right. unfold not. intros. destruct H0. contradiction. right. unfold not. intros. destruct H0. contradiction. apply inright. intros. unfold not. intros. inversion H0. intros.
+
+
+                    
+
+                                                                                                                                                                                                                                                                                                                                                                                                     intros. unfold Dual. simpl. unfold Dual in n. unfold not in n. unfold not.  intros. destruct H.  apply n in H0.  assumption. apply inright. unfold Dual. simpl. unfold not. unfold not in n. intros. destruct H1. symmetry in H1. apply n in H1.  assumption. intros. apply inright. unfold Dual. simpl. unfold not. trivial. intros. apply inright. unfold Dual. unfold not. trivial. intros. apply inright. unfold Dual. unfold not. trivial. destruct p2. intros. assert ({t0 = t1} + {t0 <> t1}). apply (eq_type_dec t0 t1). destruct H0. subst. assert (message T1 + {~ Dual (p m) p2 }). apply (runProto' p'0 p' T1 T0 (p m) p2 (protoTypeLength p'0)). destruct X. apply inleft. exact m0. apply inright. intros. unfold Dual. simpl. unfold Dual in n. unfold not in n. unfold not.  intros. destruct H0.  apply n in H1.  assumption. apply inright. unfold Dual. simpl. unfold not. unfold not in n. intros. destruct H0. symmetry in H0. apply n in H0.  assumption. intros. apply inright. unfold Dual. unfold not. trivial. intros.  apply inright. intros. unfold not. intros. inversion H0. intros. apply inright. unfold not. intros. inversion H0. intros. apply inright. unfold not. intros. inversion H0.  intros. destruct p2. destruct b. apply inright. unfold not. intros. inversion H0. apply inright. unfold not. intros. inversion H0. apply inright. unfold not. intros. inversion H0. apply inright. unfold not. intros. inversion H0.*) destruct b. destruct p2. apply inright. apply NotDual. unfold not. intros. contradiction. 
+                    apply inright. apply NotDual. unfold not. intros. contradiction.
+                    apply inright. apply NotDual. unfold not. intros. contradiction.
+                    assert ({DualT r r0} + {~ DualT r r0}). apply (DualT_dec r r0). assert ({DualT s s0} + {~ DualT s s0}). apply (DualT_dec s s0). destruct H0. destruct H1. destruct (runProto' r r0 R R0 p p2_1 (protoTypeLength r0)). left. exact m. apply inright. apply NoDecrypt. apply inright. apply NotDual. unfold not. intros. inversion H0. contradiction. apply inright. apply NotDual. unfold not. intros. inversion H0. contradiction. destruct (decrypt m k). apply p2 in m0. destruct (runProto' _ _ _ _ p m0 (protoTypeLength p')). apply inleft. exact m1. apply inright. apply NoDecrypt. apply inright. apply NoDecrypt. apply inright. apply NotDual. unfold not. intros. contradiction. destruct p2. apply inright. apply NotDual. unfold not. intros. contradiction. apply inright. apply NotDual. unfold not. intros. contradiction. apply inright. apply NotDual. unfold not. intros. contradiction. assert ({DualT r r0} + {~ DualT r r0}). apply (DualT_dec r r0). assert ({DualT s s0} + {~ DualT s s0}). apply (DualT_dec s s0). destruct H0. destruct H1. destruct (runProto' _ _ _ _ p0 p (protoTypeLength r0)). left. exact m. apply inright. apply NoDecrypt. apply inright. apply NotDual. unfold not. intros. inversion H0. contradiction. apply inright. apply NotDual. unfold not. intros. inversion H0. contradiction. destruct (decrypt m k). apply p2 in m0. destruct (runProto' _ _ _ _ p0 m0 (protoTypeLength p')). apply inleft. exact m1. destruct (decrypt m k). apply p2 in m1. destruct (runProto' _ _ _ _ p0 m1 (protoTypeLength p')). apply inleft. exact m2. apply inright. apply NoDecrypt. apply inright. apply NoDecrypt. apply inright. apply NoDecrypt. apply inright. apply NotDual. unfold not. intros. inversion H0. intros. destruct p2. apply inright. apply NotDual. unfold not. intros. inversion H0. apply inright. apply NotDual. unfold not. intros. inversion H0.
+
+                    destruct b.
+                    assert ({DualT r r0} + {~ DualT r r0}). apply (DualT_dec r r0). assert ({DualT s s0} + {~ DualT s s0}). apply (DualT_dec s s0). destruct H0. destruct H1. destruct (runProto' r r0 R R0 p p2_1 (protoTypeLength r0)). left. exact (leither _ _ m). apply inright. apply NoDecrypt. apply inright. apply NotDual. unfold not. intros. inversion H0. contradiction. apply inright. apply NotDual. unfold not. intros. inversion H0. contradiction.
+
+                    assert ({DualT r r0} + {~ DualT r r0}). apply (DualT_dec r r0). assert ({DualT s s0} + {~ DualT s s0}). apply (DualT_dec s s0). destruct H0. destruct H1. destruct (runProto' r r0 R R0 p p2_1 (protoTypeLength r0)). left. exact (leither _ _ m). apply inright. apply NoDecrypt. apply inright. apply NotDual. unfold not. intros. inversion H0. contradiction. apply inright. apply NotDual. unfold not. intros. inversion H0. contradiction. apply inright. apply NotDual. unfold not. intros. inversion H0. 
+
+                    destruct (decrypt m k). apply p2 in m0. destruct (runProto' _ _ _ _ p m0 (protoTypeLength p')). apply inleft. exact (leither _ _ m1). apply inright. apply NoDecrypt. apply inright. apply NoDecrypt. apply inright. apply NotDual. unfold not. intros. contradiction. intros. destruct (decrypt m k). destruct p2. assert (message T0 + {(protoError (p m0) (SendC m1 p2) )}). apply (runProto' _ _ _ _ (p m0) (SendC m1 p2) (protoTypeLength p'0)). destruct X. apply inleft. exact m2. apply inright. apply NoDecrypt. destruct (runProto' _ _ _ _ (p m0) (ReceiveC p0) (protoTypeLength p')). apply inleft. exact m1. apply inright. apply NoDecrypt. assert (message T0 + {(protoError (p m0) (ChoiceC b p2_1 p2_2) )}). apply (runProto' _ _ _ _ (p m0) (ChoiceC b p2_1 p2_2) (protoTypeLength p')). destruct X. apply inleft. exact m1. apply inright. apply NoDecrypt. assert (message T0 + {(protoError (p m0) (OfferC p2_1 p2_2) )}). apply (runProto' _ _ _ _ (p m0) (OfferC p2_1 p2_2) (protoTypeLength p')). destruct X. apply inleft. exact m1. apply inright. apply NoDecrypt. destruct (decrypt m1 k0). 
+
+                    assert (message T0 + {(protoError (p m0) (p0 m2 ))}). apply (runProto' _ _ _ _ (p m0) (p0 m2) (protoTypeLength p')). destruct X. apply inleft. exact m3. apply inright. apply NoDecrypt. apply inright. apply NoDecrypt. assert (message T0 + {(protoError (p m0) (ReturnC m) )}). apply (runProto' _ _ _ _ (p m0) (ReturnC m) (protoTypeLength p')). destruct X. apply inleft. exact m2. apply inright. apply NoDecrypt. apply inright. apply NoDecrypt. intros. destruct p2. apply inright. apply NotDual. unfold not. intros. contradiction. apply inright. apply NotDual. unfold not. intros. contradiction. apply inright. apply NotDual. unfold not. intros. contradiction.  apply inright. apply NotDual. unfold not. intros. contradiction. destruct (decrypt m0 k). assert (message t0 + {(protoError (ReturnC m) (p m1 ))}). apply (runProto' _ _ _ _ (ReturnC m) (p m1) (protoTypeLength p')). destruct X. apply inleft. exact m2. apply inright. apply NoDecrypt. apply inright. apply NoDecrypt. apply inleft. exact m. Defined.
+
+                    assert (message T0 + {(protoError (p m0) (p0 m2 ))}). apply (runProto' _ _ _ _ (p m0) (p0 m2) (protoTypeLength p')). destruct X. apply inleft. exact m3. apply inright. apply NoDecrypt. apply inright. apply NoDecrypt.
+
+                    contradiction. apply inright. apply NotDual. unfold not. intros. contradiction. apply inright. apply NotDual. unfold not. intros. contradiction. assert ({DualT r r0} + {~ DualT r r0}). apply (DualT_dec r r0). assert ({DualT s s0} + {~ DualT s s0}). apply (DualT_dec s s0). destruct H0. destruct H1. destruct (runProto' _ _ _ _ p0 p (protoTypeLength r0)). left. exact m. apply inright. apply NoDecrypt. apply inright. apply NotDual. unfold not. intros. inversion H0. contradiction. apply inright. apply NotDual. unfold not. intros. inversion H0. contradiction. destruct (decrypt m k). apply p2 in m0. destruct (runProto' _ _ _ _ p0 m0 (protoTypeLength p')). apply inleft. exact m1. destruct (decrypt m k). apply p2 in m1. destruct (runProto' _ _ _ _ p0 m1 (protoTypeLength p')). apply inleft. exact m2. apply inright. apply NoDecrypt. apply inright. apply NoDecrypt. apply inright. apply NoDecrypt. apply inright. apply NotDual. unfold not. intros. inversion H0. intros. destruct p2. apply inright. apply NotDual. unfold not. intros. inversion H0. apply inright. apply NotDual. unfold not. intros. inversion H0.
+
+                    
+                    unfold not in n. unfold Dual in n. apply n in d. inversion d. right. unfold not. intros. destruct H0. contradiction. right. unfold not. intros. destruct H0. contradiction.
+
+                    unfold Dual. assert ({DualT s s0} + {~ DualT s s0}). apply (DualT_dec s s0). assert ({DualT r r0} + {~ DualT r r0}). apply (DualT_dec r r0). destruct H0. destruct H1. destruct (runProto' s s0 S S0 p0 p2_2 (protoTypeLength s0)). left. exact m. unfold not in n. unfold Dual in n. apply n in d. inversion d. right. unfold not. intros. destruct H0. contradiction. right. unfold not. intros. destruct H0. contradiction. apply inright. intros. unfold not. intros. inversion H0. intros.  
+
+                    destruct p2. right. unfold not. intros. inversion H0. right. unfold not. intros. inversion H0. destruct b. unfold Dual. assert ({DualT r r0} + {~ DualT r r0}). apply (DualT_dec r r0). assert ({DualT s s0} + {~ DualT s s0}). apply (DualT_dec s s0). destruct H0. destruct H1. destruct (runProto' s s0 S S0 p0 p2_2 (protoTypeLength s0)). left. exact (reither R S m). unfold not in n. unfold Dual in n. apply n in d0. inversion d0. right. unfold not. intros. destruct H0. contradiction. right. unfold not. intros. destruct H0. contradiction. unfold Dual. assert ({DualT r r0} + {~ DualT r r0}). apply (DualT_dec r r0). assert ({DualT s s0} + {~ DualT s s0}). apply (DualT_dec s s0). destruct H0. destruct H1. destruct (runProto' r r0 R R0 p p2_1 (protoTypeLength r0)). left. exact (leither R S m). unfold not in n. unfold Dual in n. apply n in d. inversion d. right. unfold not. intros. destruct H0. contradiction. right. unfold not. intros. destruct H0. contradiction. right. unfold not. intros. inversion H0. right. unfold not. intros. inversion H0. intros. destruct p2. right. unfold not. intros. inversion H0. right. unfold not. intros. inversion H0. right. unfold not. intros. inversion H0. right. unfold not. intros. inversion H0. left. exact m. Defined.
+
+Inductive protoError {t t':protoType} {T T':type} (p1:protoExp T t) (p2:protoExp T' t') : Type :=
+| NotDual : (~ Dual p1 p2) -> protoError p1 p2
+| NoDecrypt : protoError p1 p2.
+  
+Definition runProto {t t':protoType} {T T':type} (p1:protoExp T t) (p2:protoExp T' t')
+  : (message T) + {(~ (Dual p1 p2))} := runProto' p1 p2 (protoLength p1).
+
+Definition proto3 :=
+  send (basic 1);
+  ReturnC (t:=Basic) (basic 1).
+
+Definition proto3' :=
+  x <- receive;
+  ReturnC (t:=Basic) x.
+
+Definition incPayload (m:message Basic) : (message Basic) :=
+  match m with
+  | basic n => basic (n + 1)
+  end.
+  
+Definition proto4 :=
+  x <- receive;
+  send (incPayload x);
+  ReturnC x.
+Check proto4.
+
+Definition proto5 :=
+  send (basic 1);
+  x <- receive;
+  ReturnC (t:=Basic) x.
+Check proto5.
+
+Example dual45 : Dual proto4 proto5. unfold Dual. simpl. auto.
+
+Definition proto6 :=
+  choice true EpsC
+         proto4. Check proto6.
+
+Definition proto7 :=
+  offer EpsC
+        proto5. Check proto7.
+
+Example dual67 : Dual proto6 proto7. unfold Dual. simpl. auto. Qed.
+           
+Eval compute in (runProto proto3 proto3').
+
+Eval compute in (runProto proto4 proto5).
+Eval compute in (runProto proto5 proto4).
+Eval compute in (runProto proto5 proto3).
+Eval compute in (runProto proto6 proto7). *)
+
+
+
+End try13.
